@prefix schema: <http://schema.org/> .
@prefix rdfs: <http://www.w3.org/2000/01/rdf-schema#> .
@prefix foaf: <http://xmlns.com/foaf/0.1/> .
@prefix skos: <http://www.w3.org/2004/02/skos/core#> .
@prefix dcterms: <http://purl.org/dc/terms/> .


<https://twitter.com/kidehen/status/1173666583924944896#> a schema:CreativeWork , foaf:Document ;
	schema:url <https://twitter.com/kidehen/status/1173666583924944896> ;
	schema:name "Retweet @ValaAfshar:  12 people would have gone online in India for the first time" ;
	skos:related <https://twitter.com/hashtag/India#this> , <https://twitter.com/hashtag/MarketResearch#this> , <https://twitter.com/hashtag/Economy#this> , <https://twitter.com/hashtag/GlobalEconomy#this> , <http://data.openlinksw.com/oplweb/glossary-term/India#this> , <http://data.openlinksw.com/oplweb/glossary-term/MarketResearch#this> , <http://data.openlinksw.com/oplweb/glossary-term/Economy#this> , <http://data.openlinksw.com/oplweb/glossary-term/GlobalEconomy#this> ;
	rdfs:comment "Retweet @ValaAfshar:  12 people would have gone online in India for the first time" .

<https://twitter.com/kidehen/status/1173986956205842433#> a schema:CreativeWork , foaf:Document ;
	schema:url <https://twitter.com/kidehen/status/1173986956205842433> ;
	schema:name "The #Web is mankind's ultimate #Middleware. It's #REST-ful interaction pattern is fundamentally about loose-coupling of #Data that rides the power of a #Hyperlink functioning as a #SuperKey. This platform is \"deceptively simple\" and has room for a variety of user profiles.  Retweet @judell" ;
	skos:related <https://twitter.com/hashtag/Web#this> , <https://twitter.com/hashtag/Middleware#this> , <https://twitter.com/hashtag/REST#this> , <https://twitter.com/hashtag/Data#this> , <https://twitter.com/hashtag/Hyperlink#this> , <http://ecrm.intranet.openlinksw.com/us_mis_csv#https%3A%2F%2Ftwitter.com%2Fhashtag%2FSuperKey.+%23this> , <http://data.openlinksw.com/oplweb/glossary-term/Web#this> , <http://data.openlinksw.com/oplweb/glossary-term/Middleware#this> , <http://data.openlinksw.com/oplweb/glossary-term/REST#this> , <http://data.openlinksw.com/oplweb/glossary-term/Data#this> , <http://data.openlinksw.com/oplweb/glossary-term/Hyperlink#this> , <http://data.openlinksw.com/oplweb/glossary-term/SuperKey#this> ;
	rdfs:comment "The #Web is mankind's ultimate #Middleware. It's #REST-ful interaction pattern is fundamentally about loose-coupling of #Data that rides the power of a #Hyperlink functioning as a #SuperKey. This platform is \"deceptively simple\" and has room for a variety of user profiles.  Retweet @judell" .

<https://twitter.com/kidehen/status/1174023781439954945#> a schema:CreativeWork , foaf:Document ;
	schema:url <https://twitter.com/kidehen/status/1174023781439954945> ;
	schema:name """ Replying to 
@EmekaOkoye
 
@asemota
 and 3 others
Domain Experts and App Developers collectively produce useful Apps & Services. One without the other produces a much lesser final product, 100% of the time :) """ ;
	skos:related <https://twitter.com/hashtag/Coding#this> , <https://twitter.com/hashtag/Programming#this> , <https://twitter.com/hashtag/DomainExpertise#this> , <http://data.openlinksw.com/oplweb/glossary-term/Coding#this> , <http://data.openlinksw.com/oplweb/glossary-term/Programming#this> , <http://data.openlinksw.com/oplweb/glossary-term/DomainExpertise#this> ;
	rdfs:comment """ Replying to 
@EmekaOkoye
 
@asemota
 and 3 others
Domain Experts and App Developers collectively produce useful Apps & Services. One without the other produces a much lesser final product, 100% of the time :) """ .

<https://twitter.com/shewardmills/status/1173622758435119106#> a schema:CreativeWork , foaf:Document ;
	schema:url <https://twitter.com/shewardmills/status/1173622758435119106> ;
	schema:name "EU_DataPortal:  Slovakia" ;
	skos:related <https://twitter.com/hashtag/LinkedData#this> , <https://twitter.com/hashtag/KnowledgeGraph#this> , <https://twitter.com/hashtag/VirtuosoRDBMS#this> , <http://data.openlinksw.com/oplweb/glossary-term/LinkedData#this> , <http://data.openlinksw.com/oplweb/glossary-term/KnowledgeGraph#this> , <http://data.openlinksw.com/oplweb/glossary-term/VirtuosoRDBMS#this> ;
	rdfs:comment "EU_DataPortal:  Slovakia" .

<https://twitter.com/shewardmills/status/1173940641782517760#> a schema:CreativeWork , foaf:Document ;
	schema:url <https://twitter.com/shewardmills/status/1173940641782517760> ;
	schema:name "EU_DataPortal:  Slovenia" ;
	skos:related <https://twitter.com/hashtag/LinkedData#this> , <https://twitter.com/hashtag/KnowledgeGraph#this> , <https://twitter.com/hashtag/VirtuosoRDBMS#this> , <http://data.openlinksw.com/oplweb/glossary-term/LinkedData#this> , <http://data.openlinksw.com/oplweb/glossary-term/KnowledgeGraph#this> , <http://data.openlinksw.com/oplweb/glossary-term/VirtuosoRDBMS#this> ;
	rdfs:comment "EU_DataPortal:  Slovenia" .

<https://twitter.com/dan_hmills/status/1173604327086284805#> a schema:CreativeWork , foaf:Document ;
	schema:url <https://twitter.com/dan_hmills/status/1173604327086284805> ;
	schema:name """(1/3)
Fun Fact:

You can share a SPARQL query from an @OpenLink
  Virtuoso #SPARQL Editor instance by clicking on the \"Permalink\" hyperlink ...""" ;
	skos:related <https://twitter.com/hashtag/LinkedData#this> , <https://twitter.com/hashtag/GraphDatabases#this> , <https://twitter.com/hashtag/VirtuosoRDBMS#this> , <https://twitter.com/hashtag/SPARQL#this> , <http://data.openlinksw.com/oplweb/glossary-term/LinkedData#this> , <http://data.openlinksw.com/oplweb/glossary-term/GraphDatabases#this> , <http://data.openlinksw.com/oplweb/glossary-term/VirtuosoRDBMS#this> , <http://data.openlinksw.com/oplweb/glossary-term/SPARQL#this> ;
	rdfs:comment """(1/3)
Fun Fact:

You can share a SPARQL query from an @OpenLink
  Virtuoso #SPARQL Editor instance by clicking on the \"Permalink\" hyperlink ...""" .

<https://twitter.com/kidehen/status/1174063456942723077#> a schema:CreativeWork , foaf:Document ;
	schema:url <https://twitter.com/kidehen/status/1174063456942723077> ;
	schema:name """Replying to 
@SmartCityexpo
 and 
@BCN_digital
There's also a cool #OpenData effort.

See: https://opendata-ajuntament.barcelona.cat/en/analytics""" ;
	skos:related <https://twitter.com/hashtag/OpenData#this> , <https://twitter.com/hashtag/Barcelona#this> , <http://data.openlinksw.com/oplweb/glossary-term/OpenData#this> , <http://data.openlinksw.com/oplweb/glossary-term/Barcelona#this> ;
	rdfs:comment """Replying to 
@SmartCityexpo
 and 
@BCN_digital
There's also a cool #OpenData effort.

See: https://opendata-ajuntament.barcelona.cat/en/analytics""" .

<https://twitter.com/kidehen/status/1174066642734735361#> a schema:CreativeWork , foaf:Document ;
	schema:url <https://twitter.com/kidehen/status/1174066642734735361> ;
	schema:name "DBPedia Resouce:  Mary Somerville from @barabasi:  World's first scientist" ;
	skos:related <https://twitter.com/hashtag/DidYouKnow#this> , <https://twitter.com/hashtag/Scientist#this> , <https://twitter.com/hashtag/History#this> , <https://twitter.com/hashtag/DBpedia#this> , <https://twitter.com/hashtag/LODCloud#this> , <http://data.openlinksw.com/oplweb/glossary-term/DidYouKnow#this> , <http://data.openlinksw.com/oplweb/glossary-term/Scientist#this> , <http://data.openlinksw.com/oplweb/glossary-term/History#this> , <http://data.openlinksw.com/oplweb/glossary-term/DBPedia#this> , <http://data.openlinksw.com/oplweb/glossary-term/LODCloud#this> ;
	rdfs:comment "DBPedia Resouce:  Mary Somerville from @barabasi:  World's first scientist" .

<https://twitter.com/kidehen/status/1174074694179393537#> a schema:CreativeWork , foaf:Document ;
	schema:url <https://twitter.com/kidehen/status/1174074694179393537> ;
	schema:name "#SPARQL offers a wonderful SAMPLE() aggregate function for building cool indexes that aid follow-your-nose exploration via #LinkedData docs. Example: https://tinyurl.com/y4gj4l32 Products, Restaurants, etc from a #Tourism #KnowledgeGraph." ;
	skos:related <https://twitter.com/hashtag/SPARQL#this> , <https://twitter.com/hashtag/LinkedData#this> , <https://twitter.com/hashtag/Tourism#this> , <https://twitter.com/hashtag/KnowledgeGraph.#this> , <https://twitter.com/hashtag/GraphDatabase#this> , <https://twitter.com/hashtag/SemanticWeb#this> , <http://data.openlinksw.com/oplweb/glossary-term/DidYouKnow#this> , <http://data.openlinksw.com/oplweb/glossary-term/Scientist#this> , <http://data.openlinksw.com/oplweb/glossary-term/History#this> , <http://data.openlinksw.com/oplweb/glossary-term/DBPedia#this> , <http://data.openlinksw.com/oplweb/glossary-term/LODCloud#this> ;
	rdfs:comment "#SPARQL offers a wonderful SAMPLE() aggregate function for building cool indexes that aid follow-your-nose exploration via #LinkedData docs. Example: https://tinyurl.com/y4gj4l32 Products, Restaurants, etc from a #Tourism #KnowledgeGraph." .

<https://twitter.com/kidehen/status/1174317393285439490#> a schema:CreativeWork , foaf:Document ;
	schema:url <https://twitter.com/kidehen/status/1174317393285439490> ;
	schema:name """Replying to 
@xniyi
 
@asemota
 and 4 others
Yep!

Codifying #knowledge is the key to building apps equipped with competitive longevity -- which is what the notion of a #SemanticWeb enables.

It is ultimately always about a noisy hype-driven sprint (shallow domain expertise) vs a long-tail marathon (deep domain expertise).""" ;
	skos:related <https://twitter.com/hashtag/Knowledge#this> , <https://twitter.com/hashtag/SemanticWeb#this> , <http://data.openlinksw.com/oplweb/glossary-term/Knowledge#this> , <http://data.openlinksw.com/oplweb/glossary-term/SemanticWeb#this> ;
	rdfs:comment """Replying to 
@xniyi
 
@asemota
 and 4 others
Yep!

Codifying #knowledge is the key to building apps equipped with competitive longevity -- which is what the notion of a #SemanticWeb enables.

It is ultimately always about a noisy hype-driven sprint (shallow domain expertise) vs a long-tail marathon (deep domain expertise).""" .

<https://twitter.com/kidehen/status/1174323158255591424#> a schema:CreativeWork , foaf:Document ;
	schema:url <https://twitter.com/kidehen/status/1174323158255591424> ;
	schema:name "#LinkedData is crucial to creating a #KnowledgeGraph that manifests as #SemanticWeb, period. The #Web in all of this is about a #Hyperlink-based Entity Relationship Graph that's navigable by both humans and machines using de-reference (i.e., lookups)." ;
	skos:related <https://twitter.com/hashtag/LinkedData#this> , <https://twitter.com/hashtag/KnowledgeGraph#this> , <https://twitter.com/hashtag/SemanticWeb#this> , <https://twitter.com/hashtag/Web#this> , <https://twitter.com/hashtag/Hyperlink#this> , <http://data.openlinksw.com/oplweb/glossary-term/LinkedData#this> , <http://data.openlinksw.com/oplweb/glossary-term/KnowledgeGraph#this> , <http://data.openlinksw.com/oplweb/glossary-term/SemanticWeb#this> , <http://data.openlinksw.com/oplweb/glossary-term/Web#this> , <http://data.openlinksw.com/oplweb/glossary-term/Hyperlink#this> ;
	rdfs:comment "#LinkedData is crucial to creating a #KnowledgeGraph that manifests as #SemanticWeb, period. The #Web in all of this is about a #Hyperlink-based Entity Relationship Graph that's navigable by both humans and machines using de-reference (i.e., lookups)." .

<https://twitter.com/kidehen/status/1174323829948260352#> a schema:CreativeWork , foaf:Document ;
	schema:url <https://twitter.com/kidehen/status/1174323829948260352> ;
	schema:name """@OpenLink
 has opened up a new community forum channel focused on #LinkedData with the sole aim of teaching anyone that's interested about this powerful concept via live examples.""" ;
	skos:related <https://twitter.com/hashtag/LinkedData#this> , <https://twitter.com/hashtag/GraphDatabase#this> , <https://twitter.com/hashtag/KnowledgeGraph#this> , <https://twitter.com/hashtag/SemanticWeb#this> , <https://twitter.com/hashtag/CDO#this> , <https://twitter.com/hashtag/DataOps#this> , <http://data.openlinksw.com/oplweb/glossary-term/LinkedData#this> , <http://data.openlinksw.com/oplweb/glossary-term/GraphDatabase#this> , <http://data.openlinksw.com/oplweb/glossary-term/KnowledgeGraph#this> , <http://data.openlinksw.com/oplweb/glossary-term/SemanticWeb#this> , <http://data.openlinksw.com/oplweb/glossary-term/CDO#this> , <http://data.openlinksw.com/oplweb/glossary-term/DataOps#this> ;
	rdfs:comment """@OpenLink
 has opened up a new community forum channel focused on #LinkedData with the sole aim of teaching anyone that's interested about this powerful concept via live examples.""" .

<https://twitter.com/kidehen/status/1174330675459252225#> a schema:CreativeWork , foaf:Document ;
	schema:url <https://twitter.com/kidehen/status/1174330675459252225> ;
	schema:name "Actually, here is a very basic depiction of an Entity Relationship Graph constructed in line with #LinkedData principles. #GraphDatabase #KnowledgeGraph #CDO #DataOps" ;
	skos:related <https://twitter.com/hashtag/LinkedData#this> , <https://twitter.com/hashtag/GraphDatabase#this> , <https://twitter.com/hashtag/KnowledgeGraph#this> , <https://twitter.com/hashtag/CDO#this> , <https://twitter.com/hashtag/DataOps#this> , <http://data.openlinksw.com/oplweb/glossary-term/LinkedData#this> , <http://data.openlinksw.com/oplweb/glossary-term/GraphDatabase#this> , <http://data.openlinksw.com/oplweb/glossary-term/KnowledgeGraph#this> , <http://data.openlinksw.com/oplweb/glossary-term/CDO#this> , <http://data.openlinksw.com/oplweb/glossary-term/DataOps#this> ;
	rdfs:comment "Actually, here is a very basic depiction of an Entity Relationship Graph constructed in line with #LinkedData principles. #GraphDatabase #KnowledgeGraph #CDO #DataOps" .

<https://twitter.com/kidehen/status/1174336300591304707#> a schema:CreativeWork , foaf:Document ;
	schema:url <https://twitter.com/kidehen/status/1174336300591304707> ;
	schema:name """Replying to 
@neumarcx
Folks in \"my network\" that still find the basic concepts and virtues of #LinkedData somewhat mercurial.

How do I know that? By analyzing the content of theirs tweets e.g., chatter about problems easily solved by understanding and exploiting Linked Data principles.""" ;
	skos:related <https://twitter.com/hashtag/LinkedData#this> , <http://data.openlinksw.com/oplweb/glossary-term/LinkedData#this> ;
	rdfs:comment """Replying to 
@neumarcx
Folks in \"my network\" that still find the basic concepts and virtues of #LinkedData somewhat mercurial.

How do I know that? By analyzing the content of theirs tweets e.g., chatter about problems easily solved by understanding and exploiting Linked Data principles.""" .

<https://twitter.com/kidehen/status/1174337284331753475#> a schema:CreativeWork , foaf:Document ;
	schema:url <https://twitter.com/kidehen/status/1174337284331753475> ;
	schema:name """Replying to 
@EmekaOkoye
Yes!

Basically, you simply document the problem. 

What's magical about a #SemanticWeb constructed from #LinkedData is that the Documentation == The Code :) 

A Doc is comprised of a collection of simple sentences where a #hyperlink identifies the subject, predicate, and object.""" ;
	skos:related <https://twitter.com/hashtag/SemanticWeb#this> , <https://twitter.com/hashtag/LinkedData#this> , <https://twitter.com/hashtag/Hyperlink#this> , <http://data.openlinksw.com/oplweb/glossary-term/SemanticWeb#this> , <http://data.openlinksw.com/oplweb/glossary-term/LinkedData#this> , <http://data.openlinksw.com/oplweb/glossary-term/Hyperlink#this> ;
	rdfs:comment """Replying to 
@EmekaOkoye
Yes!

Basically, you simply document the problem. 

What's magical about a #SemanticWeb constructed from #LinkedData is that the Documentation == The Code :) 

A Doc is comprised of a collection of simple sentences where a #hyperlink identifies the subject, predicate, and object.""" .

<https://twitter.com/kidehen/status/1174337722124820480#> a schema:CreativeWork , foaf:Document ;
	schema:url <https://twitter.com/kidehen/status/1174337722124820480> ;
	schema:name """Replying to 
@kidehen
 and 
@EmekaOkoye
#Fix For #Web grammer bots:

A Doc comprises a collection of simple sentences where a #hyperlink identifies the subject, predicate, and object :)""" ;
	skos:related <https://twitter.com/hashtag/Fix#this> , <https://twitter.com/hashtag/Web#this> , <https://twitter.com/hashtag/Hyperlink#this> , <https://twitter.com/hashtag/LinkedData#this> , <https://twitter.com/hashtag/SemanticWeb#this> , <http://data.openlinksw.com/oplweb/glossary-term/Fix#this> , <http://data.openlinksw.com/oplweb/glossary-term/Web#this> , <http://data.openlinksw.com/oplweb/glossary-term/Hyperlink#this> , <http://data.openlinksw.com/oplweb/glossary-term/LinkedData#this> , <http://data.openlinksw.com/oplweb/glossary-term/SemanticWeb#this> ;
	rdfs:comment """Replying to 
@kidehen
 and 
@EmekaOkoye
#Fix For #Web grammer bots:

A Doc comprises a collection of simple sentences where a #hyperlink identifies the subject, predicate, and object :)""" .

<https://twitter.com/kidehen/status/1174349289579077635#> a schema:CreativeWork , foaf:Document ;
	schema:url <https://twitter.com/kidehen/status/1174349289579077635> ;
	schema:name """Replying to 
@westurner
I hear you! 

It isn't about new Query Languages for operating on #data. It is about the very nature of #StructuredData leveraging #Web magic. 

Data silo-fication is the problem. 

I posted earlier today about a #LinkedData channel where folks can revisit the basics :)""" ;
	skos:related <https://twitter.com/hashtag/Data#this> , <https://twitter.com/hashtag/StructuredData#this> , <https://twitter.com/hashtag/Web#this> , <https://twitter.com/hashtag/LinkedData#this> , <http://data.openlinksw.com/oplweb/glossary-term/Data#this> , <http://data.openlinksw.com/oplweb/glossary-term/StructuredData#this> , <http://data.openlinksw.com/oplweb/glossary-term/Web#this> , <http://data.openlinksw.com/oplweb/glossary-term/LinkedData#this> ;
	rdfs:comment """Replying to 
@westurner
I hear you! 

It isn't about new Query Languages for operating on #data. It is about the very nature of #StructuredData leveraging #Web magic. 

Data silo-fication is the problem. 

I posted earlier today about a #LinkedData channel where folks can revisit the basics :)""" .

<https://twitter.com/kidehen/status/1174351919231524864#> a schema:CreativeWork , foaf:Document ;
	schema:url <https://twitter.com/kidehen/status/1174351919231524864> ;
	schema:name "#LinkedData is like wine. Example: http://ontologi.es/rail/void.xhtml#this That page has existed for years, its utility and importance grows as each year goes by. Same applies to the #LODCloud -- a stealthily constructed #KnowledegGraph where data is constructed using hyperlinks." ;
	skos:related <https://twitter.com/hashtag/LinkedData#this> , <https://twitter.com/hashtag/LODCloud#this> , <https://twitter.com/hashtag/KnowledegGraph#this> , <https://twitter.com/hashtag/Railways#this> , <http://data.openlinksw.com/oplweb/glossary-term/LinkedData#this> , <http://data.openlinksw.com/oplweb/glossary-term/LODCloud#this> , <http://data.openlinksw.com/oplweb/glossary-term/KnowledgeGraph#this> , <http://data.openlinksw.com/oplweb/glossary-term/Railways#this> ;
	rdfs:comment "#LinkedData is like wine. Example: http://ontologi.es/rail/void.xhtml#this That page has existed for years, its utility and importance grows as each year goes by. Same applies to the #LODCloud -- a stealthily constructed #KnowledegGraph where data is constructed using hyperlinks." .

<https://twitter.com/kidehen/status/1174356554184908800#> a schema:CreativeWork , foaf:Document ;
	schema:url <https://twitter.com/kidehen/status/1174356554184908800> ;
	schema:name """Replying to 
@AlanMorrison
 
@EmekaOkoye
 and 4 others
Good question!

Data Artisans, Subject Matter Experts (Dept. / Project owners) etc come to mind, at first blush. 

Thinking about it further, this is more to do with role evolution by way of #DataCentric skills development and refinement, IMHO.""" ;
	skos:related <https://twitter.com/hashtag/DataCentric#this> , <https://twitter.com/hashtag/LinkedData#this> , <https://twitter.com/hashtag/KnowledgeGraph#this> , <http://data.openlinksw.com/oplweb/glossary-term/DataCentric#this> , <http://data.openlinksw.com/oplweb/glossary-term/LinkedData#this> , <http://data.openlinksw.com/oplweb/glossary-term/KnowledgeGraph#this> ;
	rdfs:comment """Replying to 
@AlanMorrison
 
@EmekaOkoye
 and 4 others
Good question!

Data Artisans, Subject Matter Experts (Dept. / Project owners) etc come to mind, at first blush. 

Thinking about it further, this is more to do with role evolution by way of #DataCentric skills development and refinement, IMHO.""" .

<https://twitter.com/kidehen/status/1174358024024133633#> a schema:CreativeWork , foaf:Document ;
	schema:url <https://twitter.com/kidehen/status/1174358024024133633> ;
	schema:name """Replying to 
@davewiner
The challenge is getting to a place where app-logic and #data storage are loosely-coupled by apps (e.g., search engines).

End-users should control preferences (profile) data while apps should seek access permission.

#SolidHelps this kind of #RWW via #LinkedData :)""" ;
	skos:related <https://twitter.com/hashtag/Data#this> , <https://twitter.com/hashtag/SolidHelps#this> , <https://twitter.com/hashtag/RWW#this> , <https://twitter.com/hashtag/LinkedData#this> , <http://data.openlinksw.com/oplweb/glossary-term/Data#this> , <http://data.openlinksw.com/oplweb/glossary-term/SolidHelps#this> , <http://data.openlinksw.com/oplweb/glossary-term/RWW#this> , <http://data.openlinksw.com/oplweb/glossary-term/LinkedData#this> ;
	rdfs:comment """Replying to 
@davewiner
The challenge is getting to a place where app-logic and #data storage are loosely-coupled by apps (e.g., search engines).

End-users should control preferences (profile) data while apps should seek access permission.

#SolidHelps this kind of #RWW via #LinkedData :)""" .

<https://twitter.com/kidehen/status/1174360662656671745#> a schema:CreativeWork , foaf:Document ;
	schema:url <https://twitter.com/kidehen/status/1174360662656671745> ;
	schema:name """Replying to 
@kidehen
 
@AlanMorrison
 and 5 others
Historically, Subject Matter (or Domain) Experts are a zillion miles away from the act of #Knowledge encoding. 

Courtesy of #RDF deployed using #LinkedData principles, we can use the documentation-pattern as basis for inclusive coding.

#RDFTurtle looks like human sentences :)""" ;
	skos:related <https://twitter.com/hashtag/Knowledge#this> , <https://twitter.com/hashtag/RDF#this> , <https://twitter.com/hashtag/LinkedData#this> , <https://twitter.com/hashtag/RDFTurtle#this> , <http://data.openlinksw.com/oplweb/glossary-term/Knowledge#this> , <http://data.openlinksw.com/oplweb/glossary-term/RDF#this> , <http://data.openlinksw.com/oplweb/glossary-term/LinkedData#this> , <http://data.openlinksw.com/oplweb/glossary-term/RDFTurtle#this> ;
	rdfs:comment """Replying to 
@kidehen
 
@AlanMorrison
 and 5 others
Historically, Subject Matter (or Domain) Experts are a zillion miles away from the act of #Knowledge encoding. 

Courtesy of #RDF deployed using #LinkedData principles, we can use the documentation-pattern as basis for inclusive coding.

#RDFTurtle looks like human sentences :)""" .

<https://twitter.com/kidehen/status/1174362421546364928#> a schema:CreativeWork , foaf:Document ;
	schema:url <https://twitter.com/kidehen/status/1174362421546364928> ;
	schema:name """@datasniff
 shedding a light more light on the wine-like nature of #LinkedData demonstrated by that page about UK Railways.""" ;
	skos:related <https://twitter.com/hashtag/LinkedData#this> , <https://twitter.com/hashtag/GraphDatabase#this> , <https://twitter.com/hashtag/KnowledgeGraph#this> , <https://twitter.com/hashtag/RDFa#this> , <https://twitter.com/hashtag/HTML5#this> , <https://twitter.com/hashtag/Manchester#this> , <https://twitter.com/hashtag/Trains#this> , <http://data.openlinksw.com/oplweb/glossary-term/LinkedData#this> , <http://data.openlinksw.com/oplweb/glossary-term/GraphDatabase#this> , <http://data.openlinksw.com/oplweb/glossary-term/KnowledgeGraph#this> , <http://data.openlinksw.com/oplweb/glossary-term/RDFa#this> , <http://data.openlinksw.com/oplweb/glossary-term/HTML5#this> , <http://data.openlinksw.com/oplweb/glossary-term/Manchester#this> , <http://data.openlinksw.com/oplweb/glossary-term/Trains#this> ;
	rdfs:comment """@datasniff
 shedding a light more light on the wine-like nature of #LinkedData demonstrated by that page about UK Railways.""" .

<https://twitter.com/kidehen/status/1174365984515416066#> a schema:CreativeWork , foaf:Document ;
	schema:url <https://twitter.com/kidehen/status/1174365984515416066> ;
	schema:name "Another example that demonstrates why #LinkedData is like wine. This too has been in place for years :) UK Ordnance Survey: http://data.ordnancesurvey.co.uk" ;
	skos:related <https://twitter.com/hashtag/LinkedData#this> , <https://twitter.com/hashtag/GraphDatabase#this> , <https://twitter.com/hashtag/KnowledgeGraph#this> , <https://twitter.com/hashtag/OpenData#this> , <https://twitter.com/hashtag/SemanticWeb#this> , <https://twitter.com/hashtag/LODCloud#this> , <http://data.openlinksw.com/oplweb/glossary-term/LinkedData#this> , <http://data.openlinksw.com/oplweb/glossary-term/GraphDatabase#this> , <http://data.openlinksw.com/oplweb/glossary-term/KnowledgeGraph#this> , <http://data.openlinksw.com/oplweb/glossary-term/OpenData#this> , <http://data.openlinksw.com/oplweb/glossary-term/SemanticWeb#this> , <http://data.openlinksw.com/oplweb/glossary-term/LODCloud#this> ;
	rdfs:comment "Another example that demonstrates why #LinkedData is like wine. This too has been in place for years :) UK Ordnance Survey: http://data.ordnancesurvey.co.uk" .

<https://twitter.com/kidehen/status/1174369931825209344#> a schema:CreativeWork , foaf:Document ;
	schema:url <https://twitter.com/kidehen/status/1174369931825209344> ;
	schema:name """Replying to 
@AlanMorrison
 
@EmekaOkoye
 and 4 others
Years ago we built a #SPARQL Query Builder called #iSPARQL to do just that. 

As time went by, the simplicity of #RDFTurtle sentences reached a point where the tool was getting in the way. That's why we developed @datasniff
 and #nanotation :)""" ;
	skos:related <https://twitter.com/hashtag/SPARQL#this> , <https://twitter.com/hashtag/iSPARQL#this> , <https://twitter.com/hashtag/RDFTurtle#this> , <https://twitter.com/hashtag/Nanotation#this> , <https://twitter.com/hashtag/LinkedData#this> , <https://twitter.com/hashtag/GraphDatabase#this> , <http://data.openlinksw.com/oplweb/glossary-term/SPARQL#this> , <http://data.openlinksw.com/oplweb/glossary-term/iSPARQL#this> , <http://data.openlinksw.com/oplweb/glossary-term/RDFTurtle#this> , <http://data.openlinksw.com/oplweb/glossary-term/Nanotation#this> , <http://data.openlinksw.com/oplweb/glossary-term/LinkedData#this> , <http://data.openlinksw.com/oplweb/glossary-term/GraphDatabase#this> ;
	rdfs:comment """Replying to 
@AlanMorrison
 
@EmekaOkoye
 and 4 others
Years ago we built a #SPARQL Query Builder called #iSPARQL to do just that. 

As time went by, the simplicity of #RDFTurtle sentences reached a point where the tool was getting in the way. That's why we developed @datasniff
 and #nanotation :)""" .

<https://twitter.com/kidehen/status/1174370767183765505#> a schema:CreativeWork , foaf:Document ;
	schema:url <https://twitter.com/kidehen/status/1174370767183765505> ;
	schema:name """Replying to 
@AlanMorrison
 
@EmekaOkoye
 and 4 others
Visual UIs are good compliments. The key (as I see it) boils down to more #LinkedData tools that help end-users understand all the #KnowledgeGraph productivity magic they are missing out on. 

The #Web isn't a fluke. It's enabled by a lot of \"deceptively simple\" magic :)""" ;
	skos:related <https://twitter.com/hashtag/LinkedData#this> , <https://twitter.com/hashtag/KnowledgeGraph#this> , <https://twitter.com/hashtag/Web#this> , <http://data.openlinksw.com/oplweb/glossary-term/LinkedData#this> , <http://data.openlinksw.com/oplweb/glossary-term/KnowledgeGraph#this> , <http://data.openlinksw.com/oplweb/glossary-term/Web#this> ;
	rdfs:comment """Replying to 
@AlanMorrison
 
@EmekaOkoye
 and 4 others
Visual UIs are good compliments. The key (as I see it) boils down to more #LinkedData tools that help end-users understand all the #KnowledgeGraph productivity magic they are missing out on. 

The #Web isn't a fluke. It's enabled by a lot of \"deceptively simple\" magic :)""" .

<https://twitter.com/kidehen/status/1174371664303394817#> a schema:CreativeWork , foaf:Document ;
	schema:url <https://twitter.com/kidehen/status/1174371664303394817> ;
	schema:name """Replying to 
@EmekaOkoye
 
@AlanMorrison
 and 4 others
It's all about choice i.e., \"horses for courses\" . 

AND works better than OR i.e., whenever end-users are forced to chose one thing over another the end result is confusion. 

It took building a #SPARQL query tool to drive home the awesome power of raw #RDFTurtle sentences :)""" ;
	skos:related <https://twitter.com/hashtag/SPARQL#this> , <https://twitter.com/hashtag/RDFTurtle#this> , <http://data.openlinksw.com/oplweb/glossary-term/SPARQL#this> , <http://data.openlinksw.com/oplweb/glossary-term/RDFTurtle#this> ;
	rdfs:comment """Replying to 
@EmekaOkoye
 
@AlanMorrison
 and 4 others
It's all about choice i.e., \"horses for courses\" . 

AND works better than OR i.e., whenever end-users are forced to chose one thing over another the end result is confusion. 

It took building a #SPARQL query tool to drive home the awesome power of raw #RDFTurtle sentences :)""" .

<https://twitter.com/kidehen/status/1174373632509906946#> a schema:CreativeWork , foaf:Document ;
	schema:url <https://twitter.com/kidehen/status/1174373632509906946> ;
	schema:name "Yet another awesome example of why #LinkedData is like wine. 1. http://equipment.data.ac.uk -- equipment #KnowledgeGraph 2. http://opd.data.ac.uk -- simple setup guide for participating universities 3. https://tinyurl.com/yyd95poo -- usage demo" ;
	skos:related <https://twitter.com/hashtag/LinkedData#this> , <https://twitter.com/hashtag/KnowledgeGraph#this> , <https://twitter.com/hashtag/LODCloud#this> , <https://twitter.com/hashtag/GraphDatabase#this> , <https://twitter.com/hashtag/SemanticWeb#this> , <http://data.openlinksw.com/oplweb/glossary-term/LinkedData#this> , <http://data.openlinksw.com/oplweb/glossary-term/KnowledgeGraph#this> , <http://data.openlinksw.com/oplweb/glossary-term/LODCloud#this> , <http://data.openlinksw.com/oplweb/glossary-term/GraphDatabase#this> , <http://data.openlinksw.com/oplweb/glossary-term/SemanticWeb#this> ;
	rdfs:comment "Yet another awesome example of why #LinkedData is like wine. 1. http://equipment.data.ac.uk -- equipment #KnowledgeGraph 2. http://opd.data.ac.uk -- simple setup guide for participating universities 3. https://tinyurl.com/yyd95poo -- usage demo" .

<https://twitter.com/kidehen/status/1174375836880900096#> a schema:CreativeWork , foaf:Document ;
	schema:url <https://twitter.com/kidehen/status/1174375836880900096> ;
	schema:name """Replying to 
@kidehen
 
@AlanMorrison
 and 6 others
I forgot to add a screenshot that reveals the #SPARQL query (with #RDFTurtle in its body) generated by our #iSPARQL tool. 
""" ;
	skos:related <https://twitter.com/hashtag/SPARQL#this> , <https://twitter.com/hashtag/RDFTurtle#this> , <https://twitter.com/hashtag/iSPARQL#this> , <https://twitter.com/hashtag/GraphDatabase#this> , <https://twitter.com/hashtag/KnowledgeGraph#this> , <https://twitter.com/hashtag/SemanticWeb#this> , <http://data.openlinksw.com/oplweb/glossary-term/SPARQL#this> , <http://data.openlinksw.com/oplweb/glossary-term/RDFTurtle#this> , <http://data.openlinksw.com/oplweb/glossary-term/iSPARQL#this> , <http://data.openlinksw.com/oplweb/glossary-term/GraphDatabase#this> , <http://data.openlinksw.com/oplweb/glossary-term/KnowledgeGraph#this> , <http://data.openlinksw.com/oplweb/glossary-term/SemanticWeb#this> ;
	rdfs:comment """Replying to 
@kidehen
 
@AlanMorrison
 and 6 others
I forgot to add a screenshot that reveals the #SPARQL query (with #RDFTurtle in its body) generated by our #iSPARQL tool. 
""" .

<https://twitter.com/kidehen/status/1174377123236196360#> a schema:CreativeWork , foaf:Document ;
	schema:url <https://twitter.com/kidehen/status/1174377123236196360> ;
	schema:name """Replying to 
@AlanMorrison
 
@EmekaOkoye
 and 4 others
Over the years I've come to realize this journey is identical to the pre-#Web era when the notion of using a #hyperlink as a document identifier was quite confusing until #Mosaic unleashed the Kraken -- by revealing the magic of #HTML deployed using Linked Document Principles :)""" ;
	skos:related <https://twitter.com/hashtag/Web#this> , <https://twitter.com/hashtag/Hyperlink#this> , <https://twitter.com/hashtag/Mosaic#this> , <https://twitter.com/hashtag/HTML#this> , <http://data.openlinksw.com/oplweb/glossary-term/Web#this> , <http://data.openlinksw.com/oplweb/glossary-term/Hyperlink#this> , <http://data.openlinksw.com/oplweb/glossary-term/Mosaic#this> , <http://data.openlinksw.com/oplweb/glossary-term/HTML#this> ;
	rdfs:comment """Replying to 
@AlanMorrison
 
@EmekaOkoye
 and 4 others
Over the years I've come to realize this journey is identical to the pre-#Web era when the notion of using a #hyperlink as a document identifier was quite confusing until #Mosaic unleashed the Kraken -- by revealing the magic of #HTML deployed using Linked Document Principles :)""" .

<https://twitter.com/kidehen/status/1174382278413344768#> a schema:CreativeWork , foaf:Document ;
	schema:url <https://twitter.com/kidehen/status/1174382278413344768> ;
	schema:name """Replying to 
@kidehen
 
@AlanMorrison
 and 6 others
Demonstrating how a #SemanticWeb handles #EntityResolution (or Disparate Entity Reconciliation) is easier using the following #LinkedData:

{:i owl:sameAs :me }
WHERE
{
:i foaf:nick <@kidehen
> . 
:me foaf:nick <@kidehen
> . 
foaf:nick a owl:inverseFunctionalProperty.
}""" ;
	skos:related <https://twitter.com/hashtag/SemanticWeb#this> , <https://twitter.com/hashtag/EntityResolution#this> , <https://twitter.com/hashtag/LinkedData#this> , <http://data.openlinksw.com/oplweb/glossary-term/SemanticWeb#this> , <http://data.openlinksw.com/oplweb/glossary-term/EntityResolution#this> , <http://data.openlinksw.com/oplweb/glossary-term/LinkedData#this> ;
	rdfs:comment """Replying to 
@kidehen
 
@AlanMorrison
 and 6 others
Demonstrating how a #SemanticWeb handles #EntityResolution (or Disparate Entity Reconciliation) is easier using the following #LinkedData:

{:i owl:sameAs :me }
WHERE
{
:i foaf:nick <@kidehen
> . 
:me foaf:nick <@kidehen
> . 
foaf:nick a owl:inverseFunctionalProperty.
}""" .

<https://twitter.com/kidehen/status/1174382693326479360#> a schema:CreativeWork , foaf:Document ;
	schema:url <https://twitter.com/kidehen/status/1174382693326479360> ;
	schema:name """Replying to 
@kidehen
 
@AlanMorrison
 and 6 others
An @OpenLink
 tweet about #EntityResolution resolution that leverages a \"deceptively simple\" #HTML5-based Data Entry Form:""" ;
	skos:related <https://twitter.com/hashtag/EntityResolution#this> , <https://twitter.com/hashtag/HTML5#this> , <https://twitter.com/hashtag/GraphDatabase#this> , <https://twitter.com/hashtag/KnowledgeGraph#this> , <https://twitter.com/hashtag/LinkedData#this> , <http://data.openlinksw.com/oplweb/glossary-term/EntityResolution#this> , <http://data.openlinksw.com/oplweb/glossary-term/HTML5#this> , <http://data.openlinksw.com/oplweb/glossary-term/GraphDatabase#this> , <http://data.openlinksw.com/oplweb/glossary-term/KnowledgeGraph#this> , <http://data.openlinksw.com/oplweb/glossary-term/LinkedData#this> ;
	rdfs:comment """Replying to 
@kidehen
 
@AlanMorrison
 and 6 others
An @OpenLink
 tweet about #EntityResolution resolution that leverages a \"deceptively simple\" #HTML5-based Data Entry Form:""" .

<https://twitter.com/kidehen/status/1174430955362279424#> a schema:CreativeWork , foaf:Document ;
	schema:url <https://twitter.com/kidehen/status/1174430955362279424> ;
	schema:name """Replying to 
@AlanMorrison
 
@EmekaOkoye
 and 6 others
#screencast that demonstrate co-reference oriented reasoning & inference aided by an #Ontology:

1. https://youtu.be/H0dMM8_nQuw --  owl:sameAs 

2. https://youtu.be/IqmCVaDQ1fU --  owl:InverseFunctionalProperty""" ;
	skos:related <https://twitter.com/hashtag/Screencast#this> , <https://twitter.com/hashtag/Ontology#this> , <https://twitter.com/hashtag/GraphDatabase#this> , <https://twitter.com/hashtag/EntityResolution#this> , <https://twitter.com/hashtag/ExplainableAI#this> , <https://twitter.com/hashtag/SemanticWeb#this> , <https://twitter.com/hashtag/LinkedData#this> , <http://data.openlinksw.com/oplweb/glossary-term/Screencast#this> , <http://data.openlinksw.com/oplweb/glossary-term/Ontology#this> , <http://data.openlinksw.com/oplweb/glossary-term/GraphDatabase#this> , <http://data.openlinksw.com/oplweb/glossary-term/EntityResolution#this> , <http://data.openlinksw.com/oplweb/glossary-term/ExplainableAI#this> , <http://data.openlinksw.com/oplweb/glossary-term/SemanticWeb#this> , <http://data.openlinksw.com/oplweb/glossary-term/LinkedData#this> ;
	rdfs:comment """Replying to 
@AlanMorrison
 
@EmekaOkoye
 and 6 others
#screencast that demonstrate co-reference oriented reasoning & inference aided by an #Ontology:

1. https://youtu.be/H0dMM8_nQuw --  owl:sameAs 

2. https://youtu.be/IqmCVaDQ1fU --  owl:InverseFunctionalProperty""" .

<https://twitter.com/kidehen/status/1174431782164471809#> a schema:CreativeWork , foaf:Document ;
	schema:url <https://twitter.com/kidehen/status/1174431782164471809> ;
	schema:name """Replying to 
@kidehen
 
@AlanMorrison
 and 7 others
Live #SPARQL queries demonstrating #EntityResolution informed by Relationship Type Semantics defined in an #Ontology:

1. https://tinyurl.com/y3xkfp42 -- with reasoning & inference

2. https://tinyurl.com/y6m76nmf -- without""" ;
	skos:related <https://twitter.com/hashtag/SPARQL#this> , <https://twitter.com/hashtag/EntityResolution#this> , <https://twitter.com/hashtag/Ontology#this> , <https://twitter.com/hashtag/GraphDatabase#this> , <https://twitter.com/hashtag/KnowledgeGraph#this> , <https://twitter.com/hashtag/SemanticWeb#this> , <https://twitter.com/hashtag/LinkedData#this> , <https://twitter.com/hashtag/AI#this> , <https://twitter.com/hashtag/ML#this> , <http://data.openlinksw.com/oplweb/glossary-term/SPARQL#this> , <http://data.openlinksw.com/oplweb/glossary-term/EntityResolution#this> , <http://data.openlinksw.com/oplweb/glossary-term/Ontology#this> , <http://data.openlinksw.com/oplweb/glossary-term/GraphDatabase#this> , <http://data.openlinksw.com/oplweb/glossary-term/KnowledgeGraph#this> , <http://data.openlinksw.com/oplweb/glossary-term/SemanticWeb#this> , <http://data.openlinksw.com/oplweb/glossary-term/LinkedData#this> , <http://data.openlinksw.com/oplweb/glossary-term/AI#this> , <http://data.openlinksw.com/oplweb/glossary-term/ML#this> ;
	rdfs:comment """Replying to 
@kidehen
 
@AlanMorrison
 and 7 others
Live #SPARQL queries demonstrating #EntityResolution informed by Relationship Type Semantics defined in an #Ontology:

1. https://tinyurl.com/y3xkfp42 -- with reasoning & inference

2. https://tinyurl.com/y6m76nmf -- without""" .

<https://twitter.com/kidehen/status/1174441226533244928#> a schema:CreativeWork , foaf:Document ;
	schema:url <https://twitter.com/kidehen/status/1174441226533244928> ;
	schema:name "Retweet @datapatterns:  How do we add structured data to an existing document or file?" ;
	skos:related <https://twitter.com/hashtag/LinkedData#this> , <https://twitter.com/hashtag/KnowledgeGraph#this> , <https://twitter.com/hashtag/SemanticWeb#this> , <https://twitter.com/hashtag/Metadata#this> , <http://data.openlinksw.com/oplweb/glossary-term/EntityResolution#this> , <http://data.openlinksw.com/oplweb/glossary-term/HTML5#this> , <http://data.openlinksw.com/oplweb/glossary-term/GraphDatabase#this> , <http://data.openlinksw.com/oplweb/glossary-term/KnowledgeGraph#this> , <http://data.openlinksw.com/oplweb/glossary-term/LinkedData#this> ;
	rdfs:comment "Retweet @datapatterns:  How do we add structured data to an existing document or file?" .

<https://twitter.com/kidehen/status/1174459868759113728#> a schema:CreativeWork , foaf:Document ;
	schema:url <https://twitter.com/kidehen/status/1174459868759113728> ;
	schema:name "Retweet @karima_rafes:  Linked Open EP data of European Patent Office" ;
	skos:related <https://twitter.com/hashtag/KnowledgeGraph#this> , <https://twitter.com/hashtag/GraphDatabase#this> , <https://twitter.com/hashtag/SemanticWeb#this> , <https://twitter.com/hashtag/OpenData#this> , <https://twitter.com/hashtag/DataScience#this> , <https://twitter.com/hashtag/SPARQL#this> , <http://data.openlinksw.com/oplweb/glossary-term/KnowledgeGraph#this> , <http://data.openlinksw.com/oplweb/glossary-term/GraphDatabase#this> , <http://data.openlinksw.com/oplweb/glossary-term/SemanticWeb#this> , <http://data.openlinksw.com/oplweb/glossary-term/OpenData#this> , <http://data.openlinksw.com/oplweb/glossary-term/DataScience#this> , <http://data.openlinksw.com/oplweb/glossary-term/SPARQL#this> ;
	rdfs:comment "Retweet @karima_rafes:  Linked Open EP data of European Patent Office" .

<https://twitter.com/kidehen/status/1174460357701722113#> a schema:CreativeWork , foaf:Document ;
	schema:url <https://twitter.com/kidehen/status/1174460357701722113> ;
	schema:name "Retweet @saleem_muhamad:  Now generate real-data #SPARQL #benchmarks of your choice" ;
	skos:related <https://twitter.com/hashtag/Benchmark#this> , <https://twitter.com/hashtag/GraphDatabase#this> , <https://twitter.com/hashtag/NoSQL#this> , <https://twitter.com/hashtag/DBMS#this> , <https://twitter.com/hashtag/SPARQL#this> , <http://data.openlinksw.com/oplweb/glossary-term/Benchmark#this> , <http://data.openlinksw.com/oplweb/glossary-term/GraphDatabase#this> , <http://data.openlinksw.com/oplweb/glossary-term/NoSQL#this> , <http://data.openlinksw.com/oplweb/glossary-term/DBMS#this> , <http://data.openlinksw.com/oplweb/glossary-term/SPARQL#this> ;
	rdfs:comment "Retweet @saleem_muhamad:  Now generate real-data #SPARQL #benchmarks of your choice" .

<https://twitter.com/kidehen/status/1174460533862535179#> a schema:CreativeWork , foaf:Document ;
	schema:url <https://twitter.com/kidehen/status/1174460533862535179> ;
	schema:name "Retweet @karima_rafes:  HM Land Registry Open Data" ;
	skos:related <https://twitter.com/hashtag/GraphDatabase#this> , <https://twitter.com/hashtag/KnowledgeGraph#this> , <https://twitter.com/hashtag/LODCloud#this> , <http://data.openlinksw.com/oplweb/glossary-term/GraphDatabase#this> , <http://data.openlinksw.com/oplweb/glossary-term/KnowledgeGraph#this> , <http://data.openlinksw.com/oplweb/glossary-term/LODCloud#this> ;
	rdfs:comment "Retweet @karima_rafes:  HM Land Registry Open Data" .

<https://twitter.com/kidehen/status/1174460896426516482#> a schema:CreativeWork , foaf:Document ;
	schema:url <https://twitter.com/kidehen/status/1174460896426516482> ;
	schema:name """Retweet @karima_rafes:  Share, discover and reuse the #LinkedData has never been easier with http://linkedwiki.com

Today, there are 544 #SPARQL queries""" ;
	skos:related <https://twitter.com/hashtag/LinkedData#this> , <https://twitter.com/hashtag/SPARQL#this> , <https://twitter.com/hashtag/LOD#this> , <https://twitter.com/hashtag/KnowledgeGraph#this> , <http://ecrm.intranet.openlinksw.com/us_mis_csv#https%3A%2F%2Ftwitter.com%2Fhashtag%2FWikidata%0AGraphDatabase%23this> , <http://ecrm.intranet.openlinksw.com/us_mis_csv#https%3A%2F%2Ftwitter.com%2Fhashtag%2FNoSQL%0ASemanticWeb%23this> , <http://data.openlinksw.com/oplweb/glossary-term/LinkedData#this> , <http://data.openlinksw.com/oplweb/glossary-term/SPARQL#this> , <http://data.openlinksw.com/oplweb/glossary-term/LOD#this> , <http://data.openlinksw.com/oplweb/glossary-term/KnowledgeGraph#this> , <http://data.openlinksw.com/oplweb/glossary-term/Wikidata#this> , <http://data.openlinksw.com/oplweb/glossary-term/GraphDatabase#this> , <http://data.openlinksw.com/oplweb/glossary-term/NoSQL#this> , <http://data.openlinksw.com/oplweb/glossary-term/SemanticWeb#this> ;
	rdfs:comment """Retweet @karima_rafes:  Share, discover and reuse the #LinkedData has never been easier with http://linkedwiki.com

Today, there are 544 #SPARQL queries""" .

<https://twitter.com/kidehen/status/1174462290973773824#> a schema:CreativeWork , foaf:Document ;
	schema:url <https://twitter.com/kidehen/status/1174462290973773824> ;
	schema:name "Using #SPARQL to produce a list of SPARQL Query Service endpoints: [1] https://tinyurl.com/yxg4fmcx -- #URIBurner [2] https://w.wiki/8an -- #Wikidata Ultimately, we need a cleaned up list of functioning endpoints for better #LODCloud exploration." ;
	skos:related <https://twitter.com/hashtag/SPARQL#this> , <https://twitter.com/hashtag/URIBurner#this> , <https://twitter.com/hashtag/Wikidata#this> , <https://twitter.com/hashtag/LODCloud#this> , <https://twitter.com/hashtag/NoSQL#this> , <https://twitter.com/hashtag/GraphDatabase#this> , <http://data.openlinksw.com/oplweb/glossary-term/SPARQL#this> , <http://data.openlinksw.com/oplweb/glossary-term/URIBurner#this> , <http://data.openlinksw.com/oplweb/glossary-term/Wikidata#this> , <http://data.openlinksw.com/oplweb/glossary-term/LODCloud#this> , <http://data.openlinksw.com/oplweb/glossary-term/NoSQL#this> , <http://data.openlinksw.com/oplweb/glossary-term/GraphDatabase#this> ;
	rdfs:comment "Using #SPARQL to produce a list of SPARQL Query Service endpoints: [1] https://tinyurl.com/yxg4fmcx -- #URIBurner [2] https://w.wiki/8an -- #Wikidata Ultimately, we need a cleaned up list of functioning endpoints for better #LODCloud exploration." .

<https://twitter.com/kidehen/status/1174482992628215809#> a schema:CreativeWork , foaf:Document ;
	schema:url <https://twitter.com/kidehen/status/1174482992628215809> ;
	schema:name """Looking at some #Nigeria focused #KnowledgeGraph:

[1] https://tinyurl.com/y63tmgqv -- #PivotViewer Report 
[2] https://tinyurl.com/y352vjer -- #SPARQL Query Editor.

Re #2 an #HTTP #URI provides access to query code behind the report.""" ;
	skos:related <https://twitter.com/hashtag/Nigeria#this> , <https://twitter.com/hashtag/KnowledgeGraph#this> , <https://twitter.com/hashtag/PivotViewer#this> , <https://twitter.com/hashtag/SPARQL#this> , <https://twitter.com/hashtag/HTTP#this> , <https://twitter.com/hashtag/URI#this> , <https://twitter.com/hashtag/GraphDatabase#this> , <https://twitter.com/hashtag/Meshup#this> , <https://twitter.com/hashtag/SemanticWeb#this> , <https://twitter.com/hashtag/LinkedData#this> , <http://data.openlinksw.com/oplweb/glossary-term/Nigeria#this> , <http://data.openlinksw.com/oplweb/glossary-term/KnowledgeGraph#this> , <http://data.openlinksw.com/oplweb/glossary-term/PivotViewer#this> , <http://data.openlinksw.com/oplweb/glossary-term/SPARQL#this> , <http://data.openlinksw.com/oplweb/glossary-term/HTTP#this> , <http://data.openlinksw.com/oplweb/glossary-term/URI#this> , <http://data.openlinksw.com/oplweb/glossary-term/GraphDatabase#this> , <http://data.openlinksw.com/oplweb/glossary-term/Meshup#this> , <http://data.openlinksw.com/oplweb/glossary-term/SemanticWeb#this> , <http://data.openlinksw.com/oplweb/glossary-term/LinkedData#this> ;
	rdfs:comment """Looking at some #Nigeria focused #KnowledgeGraph:

[1] https://tinyurl.com/y63tmgqv -- #PivotViewer Report 
[2] https://tinyurl.com/y352vjer -- #SPARQL Query Editor.

Re #2 an #HTTP #URI provides access to query code behind the report.""" .

<https://twitter.com/kidehen/status/1174485027582857216#> a schema:CreativeWork , foaf:Document ;
	schema:url <https://twitter.com/kidehen/status/1174485027582857216> ;
	schema:name """Here are links to the same #SPARQL query via a basic #HTML doc.

[1] https://tinyurl.com/y69wdl2z -- Query Results 

[2] https://tinyurl.com/y68pkkg6 -- Query Definition 

You can even use @datasniff
 to expose a query editor too! All due to #HTTP #URI magic!""" ;
	skos:related <https://twitter.com/hashtag/SPARQL#this> , <https://twitter.com/hashtag/HTML#this> , <https://twitter.com/hashtag/HTTP#this> , <https://twitter.com/hashtag/URI#this> , <https://twitter.com/hashtag/GraphDatabase#this> , <https://twitter.com/hashtag/LinkedData#this> , <http://data.openlinksw.com/oplweb/glossary-term/SPARQL#this> , <http://data.openlinksw.com/oplweb/glossary-term/HTML#this> , <http://data.openlinksw.com/oplweb/glossary-term/HTTP#this> , <http://data.openlinksw.com/oplweb/glossary-term/URI#this> , <http://data.openlinksw.com/oplweb/glossary-term/GraphDatabase#this> , <http://data.openlinksw.com/oplweb/glossary-term/LinkedData#this> ;
	rdfs:comment """Here are links to the same #SPARQL query via a basic #HTML doc.

[1] https://tinyurl.com/y69wdl2z -- Query Results 

[2] https://tinyurl.com/y68pkkg6 -- Query Definition 

You can even use @datasniff
 to expose a query editor too! All due to #HTTP #URI magic!""" .

<https://twitter.com/kidehen/status/1174491992933490688#> a schema:CreativeWork , foaf:Document ;
	schema:url <https://twitter.com/kidehen/status/1174491992933490688> ;
	schema:name """Replying to 
@kidehen
 and 
@datasniff
#LinkedData is also accessible to #ODBC, #JDBC, #DotNet, and #OLEDB apps and services via #SQL (using #SPASQL).

Benefit? 
You don't have to \"rip and replace\" existing investments in order to harness the magic of a #KnowledgeGraph!""" ;
	skos:related <https://twitter.com/hashtag/LinkedData#this> , <https://twitter.com/hashtag/ODBC#this> , <https://twitter.com/hashtag/JDBC#this> , <https://twitter.com/hashtag/DotNet#this> , <https://twitter.com/hashtag/OLEDB#this> , <https://twitter.com/hashtag/SQL#this> , <https://twitter.com/hashtag/SPASQL#this> , <https://twitter.com/hashtag/KnowledgeGraph!#this> , <https://twitter.com/hashtag/CDO#this> , <https://twitter.com/hashtag/CIO#this> , <https://twitter.com/hashtag/DataOps#this> , <https://twitter.com/hashtag/CTO#this> , <https://twitter.com/hashtag/GraphDatabase#this> , <https://twitter.com/hashtag/NoSQL#this> , <http://data.openlinksw.com/oplweb/glossary-term/LinkedData#this> , <http://data.openlinksw.com/oplweb/glossary-term/ODBC#this> , <http://data.openlinksw.com/oplweb/glossary-term/JDBC#this> , <http://data.openlinksw.com/oplweb/glossary-term/DotNet#this> , <http://data.openlinksw.com/oplweb/glossary-term/OLEDB#this> , <http://data.openlinksw.com/oplweb/glossary-term/SQL#this> , <http://data.openlinksw.com/oplweb/glossary-term/SPASQL#this> , <http://data.openlinksw.com/oplweb/glossary-term/KnowledgeGraph#this> , <http://data.openlinksw.com/oplweb/glossary-term/CDO#this> , <http://data.openlinksw.com/oplweb/glossary-term/CIO#this> , <http://data.openlinksw.com/oplweb/glossary-term/DataOps#this> , <http://data.openlinksw.com/oplweb/glossary-term/CTO#this> , <http://data.openlinksw.com/oplweb/glossary-term/GraphDatabase#this> , <http://data.openlinksw.com/oplweb/glossary-term/NoSQL#this> ;
	rdfs:comment """Replying to 
@kidehen
 and 
@datasniff
#LinkedData is also accessible to #ODBC, #JDBC, #DotNet, and #OLEDB apps and services via #SQL (using #SPASQL).

Benefit? 
You don't have to \"rip and replace\" existing investments in order to harness the magic of a #KnowledgeGraph!""" .

<https://twitter.com/kidehen/status/1174680808315129856#> a schema:CreativeWork , foaf:Document ;
	schema:url <https://twitter.com/kidehen/status/1174680808315129856> ;
	schema:name """Replying to 
@csarven
You meant to say:

HG: And how it will be published as #LinkedData, I hope.
@kidehen
: I don't know any other way.
HG: I know - I thought I would feed you that line :-)""" ;
	skos:related <https://twitter.com/hashtag/LinkedData#this> , <http://data.openlinksw.com/oplweb/glossary-term/LinkedData#this> ;
	rdfs:comment """Replying to 
@csarven
You meant to say:

HG: And how it will be published as #LinkedData, I hope.
@kidehen
: I don't know any other way.
HG: I know - I thought I would feed you that line :-)""" .

<https://twitter.com/kidehen/status/1174686636212404225#> a schema:CreativeWork , foaf:Document ;
	schema:url <https://twitter.com/kidehen/status/1174686636212404225> ;
	schema:name """Replying to 
@hyperir
 
@albertmeronyo
 and 
@Deloitte
@datasniff
 also reveals the fact that @Deloitte
 is also putting #LinkedData to practical use. For instance, their #Jobs  page deploys a #KnowledgeGraph via #HTML using terms from the #SchemaOrg #Ontology. 

I can query that page using #SPARQL :) """ ;
	skos:related <https://twitter.com/hashtag/LinkedData#this> , <https://twitter.com/hashtag/Jobs#this> , <https://twitter.com/hashtag/KnowledgeGraph#this> , <https://twitter.com/hashtag/HTML#this> , <https://twitter.com/hashtag/SchemaOrg#this> , <https://twitter.com/hashtag/Ontology#this> , <https://twitter.com/hashtag/SPARQL#this> , <https://twitter.com/hashtag/GraphDatabase#this> , <https://twitter.com/hashtag/SemanticWeb#this> , <https://twitter.com/hashtag/CDO#this> , <http://data.openlinksw.com/oplweb/glossary-term/LinkedData#this> , <http://data.openlinksw.com/oplweb/glossary-term/Jobs#this> , <http://data.openlinksw.com/oplweb/glossary-term/KnowledgeGraph#this> , <http://data.openlinksw.com/oplweb/glossary-term/HTML#this> , <http://data.openlinksw.com/oplweb/glossary-term/SchemaOrg#this> , <http://data.openlinksw.com/oplweb/glossary-term/Ontology#this> , <http://data.openlinksw.com/oplweb/glossary-term/SPARQL#this> , <http://data.openlinksw.com/oplweb/glossary-term/GraphDatabase#this> , <http://data.openlinksw.com/oplweb/glossary-term/SemanticWeb#this> , <http://data.openlinksw.com/oplweb/glossary-term/CDO#this> ;
	rdfs:comment """Replying to 
@hyperir
 
@albertmeronyo
 and 
@Deloitte
@datasniff
 also reveals the fact that @Deloitte
 is also putting #LinkedData to practical use. For instance, their #Jobs  page deploys a #KnowledgeGraph via #HTML using terms from the #SchemaOrg #Ontology. 

I can query that page using #SPARQL :) """ .

<https://twitter.com/kidehen/status/1174691119755661315#> a schema:CreativeWork , foaf:Document ;
	schema:url <https://twitter.com/kidehen/status/1174691119755661315> ;
	schema:name """Replying to 
@kidehen
 
@hyperir
 and 3 others
#SPARQL query results page for this #Job #Offer deployed as a #KnowledgeGraph embedded in an #HTML doc:

[1] http://linkeddata.uriburner.com/sparql?default-graph-uri=&query=DEFINE+get%3Asoft+%22soft%22%0D%0A%0D%0ASELECT+%28SAMPLE%28%3Fs%29+AS+%3Fsample%29+%28COUNT%281%29+AS+%3Fcount%29++%28%3Fo+AS+%3FentityType%29+%3FentityTypeLabel%0D%0AWHERE+%7B%0D%0A++++++++GRAPH+%3Chttps%3A%2F%2Fwerkenbijdeloitte.nl%2Fvacatures%2Fknowledge-graph-specialist-e777989%3E+%0D%0A+++++++++++++%7B+%3Fs+a+%3Fo.%0D%0A+++++++++++++++FILTER+%28isIRI%28%3Fs%29%29%0D%0A+++++++++++++%7D+%0D%0A++++++++%23+FILTER+%28%21+CONTAINS%28STR%28%3Fo%29%2C%22Statement%22%29%29%0D%0A+++++++GRAPH+%3Fg+%7B%3Fo+rdfs%3Alabel+%3FentityTypeLabel+.%7D++%0D%0A++++++%7D+%0D%0AGROUP+BY+%3Fo+%3FentityTypeLabel%0D%0AORDER+BY+DESC+%28%3Fcount%29%0D%0A%0D%0A&should-sponge=&format=text%2Fx-html%2Btr&CXML_redir_for_subjs=121&CXML_redir_for_hrefs=&timeout=30000000


[2] http://linkeddata.uriburner.com/describe/?url=https%3A%2F%2Fwerkenbijdeloitte.nl%2Fvacatures%2Fknowledge-graph-specialist-e777989&distinct=1 -- Sample Entity Description.""" ;
	skos:related <https://twitter.com/hashtag/SPARQL#this> , <https://twitter.com/hashtag/Job#this> , <https://twitter.com/hashtag/Offer#this> , <https://twitter.com/hashtag/KnowledgeGraph#this> , <https://twitter.com/hashtag/HTML#this> , <https://twitter.com/hashtag/GraphDatabase#this> , <https://twitter.com/hashtag/LinkedData#this> , <https://twitter.com/hashtag/SemanticWeb#this> , <https://twitter.com/hashtag/HR#this> , <https://twitter.com/hashtag/SSEO#this> , <https://twitter.com/hashtag/CDO#this> , <https://twitter.com/hashtag/DataOps#this> , <https://twitter.com/hashtag/SchemaOrg#this> , <http://data.openlinksw.com/oplweb/glossary-term/SPARQL#this> , <http://data.openlinksw.com/oplweb/glossary-term/Job#this> , <http://data.openlinksw.com/oplweb/glossary-term/Offer#this> , <http://data.openlinksw.com/oplweb/glossary-term/KnowledgeGraph#this> , <http://data.openlinksw.com/oplweb/glossary-term/HTML#this> , <http://data.openlinksw.com/oplweb/glossary-term/GraphDatabase#this> , <http://data.openlinksw.com/oplweb/glossary-term/LinkedData#this> , <http://data.openlinksw.com/oplweb/glossary-term/SemanticWeb#this> , <http://data.openlinksw.com/oplweb/glossary-term/HR#this> , <http://data.openlinksw.com/oplweb/glossary-term/SSEO#this> , <http://data.openlinksw.com/oplweb/glossary-term/CDO#this> , <http://data.openlinksw.com/oplweb/glossary-term/DataOps#this> , <http://data.openlinksw.com/oplweb/glossary-term/SchemaOrg#this> ;
	rdfs:comment """Replying to 
@kidehen
 
@hyperir
 and 3 others
#SPARQL query results page for this #Job #Offer deployed as a #KnowledgeGraph embedded in an #HTML doc:

[1] http://linkeddata.uriburner.com/sparql?default-graph-uri=&query=DEFINE+get%3Asoft+%22soft%22%0D%0A%0D%0ASELECT+%28SAMPLE%28%3Fs%29+AS+%3Fsample%29+%28COUNT%281%29+AS+%3Fcount%29++%28%3Fo+AS+%3FentityType%29+%3FentityTypeLabel%0D%0AWHERE+%7B%0D%0A++++++++GRAPH+%3Chttps%3A%2F%2Fwerkenbijdeloitte.nl%2Fvacatures%2Fknowledge-graph-specialist-e777989%3E+%0D%0A+++++++++++++%7B+%3Fs+a+%3Fo.%0D%0A+++++++++++++++FILTER+%28isIRI%28%3Fs%29%29%0D%0A+++++++++++++%7D+%0D%0A++++++++%23+FILTER+%28%21+CONTAINS%28STR%28%3Fo%29%2C%22Statement%22%29%29%0D%0A+++++++GRAPH+%3Fg+%7B%3Fo+rdfs%3Alabel+%3FentityTypeLabel+.%7D++%0D%0A++++++%7D+%0D%0AGROUP+BY+%3Fo+%3FentityTypeLabel%0D%0AORDER+BY+DESC+%28%3Fcount%29%0D%0A%0D%0A&should-sponge=&format=text%2Fx-html%2Btr&CXML_redir_for_subjs=121&CXML_redir_for_hrefs=&timeout=30000000


[2] http://linkeddata.uriburner.com/describe/?url=https%3A%2F%2Fwerkenbijdeloitte.nl%2Fvacatures%2Fknowledge-graph-specialist-e777989&distinct=1 -- Sample Entity Description.""" .

<https://twitter.com/kidehen/status/1174692136459087874#> a schema:CreativeWork , foaf:Document ;
	schema:url <https://twitter.com/kidehen/status/1174692136459087874> ;
	schema:name """Replying to 
@kidehen
 
@hyperir
 and 3 others
How did I query a #Jobs posting page just like any other Table/Graph in a conventional #DBMS? 

There's a #Hyperlink for answering that question:""" ;
	skos:related <https://twitter.com/hashtag/Jobs#this> , <https://twitter.com/hashtag/DBMS#this> , <https://twitter.com/hashtag/Hyperlink#this> , <https://twitter.com/hashtag/LinkedData#this> , <https://twitter.com/hashtag/GraphDatabase#this> , <https://twitter.com/hashtag/SPARQL#this> , <https://twitter.com/hashtag/KnowledgeGraph#this> , <https://twitter.com/hashtag/SemanticWeb#this> , <https://twitter.com/hashtag/DataOps#this> , <https://twitter.com/hashtag/ConnectedData#this> , <http://data.openlinksw.com/oplweb/glossary-term/Jobs#this> , <http://data.openlinksw.com/oplweb/glossary-term/DBMS#this> , <http://data.openlinksw.com/oplweb/glossary-term/LinkedData#this> , <http://data.openlinksw.com/oplweb/glossary-term/GraphDatabase#this> , <http://data.openlinksw.com/oplweb/glossary-term/SPARQL#this> , <http://data.openlinksw.com/oplweb/glossary-term/KnowledgeGraph#this> , <http://data.openlinksw.com/oplweb/glossary-term/SemanticWeb#this> , <http://data.openlinksw.com/oplweb/glossary-term/DataOps#this> , <http://data.openlinksw.com/oplweb/glossary-term/ConnectedData#this> ;
	rdfs:comment """Replying to 
@kidehen
 
@hyperir
 and 3 others
How did I query a #Jobs posting page just like any other Table/Graph in a conventional #DBMS? 

There's a #Hyperlink for answering that question:""" .

<https://twitter.com/kidehen/status/1174694869798969344#> a schema:CreativeWork , foaf:Document ;
	schema:url <https://twitter.com/kidehen/status/1174694869798969344> ;
	schema:name """Replying to 
@kidehen
 
@danbri
 and 10 others
Found another #DBMS comparison that sheds light on both the #RDF and proprietary #GraphDatabase genres. 

See: https://mitre.org/sites/default/files/publications/pr-15-2949-ETL-from%20-RDF-to-property-graph_0.pdf
 [#PDF] .

#SPARQL #Cypher #Gremlin #NoSQL #CDO
#CIO #CTO #CMO

/ht @atomgraphhq""" ;
	skos:related <https://twitter.com/hashtag/DBMS#this> , <https://twitter.com/hashtag/RDF#this> , <https://twitter.com/hashtag/GraphDatabase#this> , <https://twitter.com/hashtag/PDF#this> , <https://twitter.com/hashtag/SPARQL#this> , <https://twitter.com/hashtag/Cypher#this> , <https://twitter.com/hashtag/Gremlin#this> , <https://twitter.com/hashtag/NoSQL#this> , <http://ecrm.intranet.openlinksw.com/us_mis_csv#https%3A%2F%2Ftwitter.com%2Fhashtag%2FCDO%0ACIO%23this> , <https://twitter.com/hashtag/CTO#this> , <https://twitter.com/hashtag/CMO#this> , <http://data.openlinksw.com/oplweb/glossary-term/DBMS#this> , <http://data.openlinksw.com/oplweb/glossary-term/RDF#this> , <http://data.openlinksw.com/oplweb/glossary-term/GraphDatabase#this> , <http://data.openlinksw.com/oplweb/glossary-term/PDF#this> , <http://data.openlinksw.com/oplweb/glossary-term/SPARQL#this> , <http://data.openlinksw.com/oplweb/glossary-term/Cypher#this> , <http://data.openlinksw.com/oplweb/glossary-term/Gremlin#this> , <http://data.openlinksw.com/oplweb/glossary-term/NoSQL#this> , <http://data.openlinksw.com/oplweb/glossary-term/CDO#this> , <http://data.openlinksw.com/oplweb/glossary-term/CIO#this> , <http://data.openlinksw.com/oplweb/glossary-term/CTO#this> , <http://data.openlinksw.com/oplweb/glossary-term/CMO#this> ;
	rdfs:comment """Replying to 
@kidehen
 
@danbri
 and 10 others
Found another #DBMS comparison that sheds light on both the #RDF and proprietary #GraphDatabase genres. 

See: https://mitre.org/sites/default/files/publications/pr-15-2949-ETL-from%20-RDF-to-property-graph_0.pdf
 [#PDF] .

#SPARQL #Cypher #Gremlin #NoSQL #CDO
#CIO #CTO #CMO

/ht @atomgraphhq""" .

<https://twitter.com/kidehen/status/1174709551683297280#> a schema:CreativeWork , foaf:Document ;
	schema:url <https://twitter.com/kidehen/status/1174709551683297280> ;
	schema:name """Replying to 
@kidehen
 
@danbri
 and 11 others
So the key issue against #RDF #GraphDatabase genre is this vague issue about pragmatism i.e., despite #LODCloud the following is theoretical?

Entity Relationship Graph where every entity and entity relationship type is unambiguously identified by a #Hyperlink i.e., #LinkedData.""" ;
	skos:related <https://twitter.com/hashtag/RDF#this> , <https://twitter.com/hashtag/GraphDatabase#this> , <https://twitter.com/hashtag/LODCloud#this> , <https://twitter.com/hashtag/Hyperlink#this> , <https://twitter.com/hashtag/LinkedData.#this> , <http://data.openlinksw.com/oplweb/glossary-term/Jobs#this> , <http://data.openlinksw.com/oplweb/glossary-term/DBMS#this> , <http://data.openlinksw.com/oplweb/glossary-term/LinkedData#this> , <http://data.openlinksw.com/oplweb/glossary-term/GraphDatabase#this> , <http://data.openlinksw.com/oplweb/glossary-term/SPARQL#this> , <http://data.openlinksw.com/oplweb/glossary-term/KnowledgeGraph#this> , <http://data.openlinksw.com/oplweb/glossary-term/SemanticWeb#this> , <http://data.openlinksw.com/oplweb/glossary-term/DataOps#this> , <http://data.openlinksw.com/oplweb/glossary-term/ConnectedData#this> ;
	rdfs:comment """Replying to 
@kidehen
 
@danbri
 and 11 others
So the key issue against #RDF #GraphDatabase genre is this vague issue about pragmatism i.e., despite #LODCloud the following is theoretical?

Entity Relationship Graph where every entity and entity relationship type is unambiguously identified by a #Hyperlink i.e., #LinkedData.""" .

<https://twitter.com/shewardmills/status/1174218843344031747#> a schema:CreativeWork , foaf:Document ;
	schema:url <https://twitter.com/shewardmills/status/1174218843344031747> ;
	schema:name "@EU_DataPortal:  Spain" ;
	skos:related <https://twitter.com/hashtag/LinkedData#this> , <https://twitter.com/hashtag/KnowledgeGraph#this> , <http://ecrm.intranet.openlinksw.com/us_mis_csv#https%3A%2F%2Ftwitter.com%2Fhashtag%2FVirtuosoRDBMS+%23this> , <https://twitter.com/hashtag/OpenData#this> , <https://twitter.com/hashtag/Dataset#this> , <http://data.openlinksw.com/oplweb/glossary-term/LinkedData#this> , <http://data.openlinksw.com/oplweb/glossary-term/KnowledgeGraph#this> , <http://data.openlinksw.com/oplweb/glossary-term/VirtuosoRDBMS#this> , <http://data.openlinksw.com/oplweb/glossary-term/OpenData#this> , <http://data.openlinksw.com/oplweb/glossary-term/Dataset#this> ;
	rdfs:comment "@EU_DataPortal:  Spain" .

<https://twitter.com/shewardmills/status/1174321958068137984#> a schema:CreativeWork , foaf:Document ;
	schema:url <https://twitter.com/shewardmills/status/1174321958068137984> ;
	schema:name """Here is  @OpenLink
 weekly recap of some of last weeks activities covering a range of topics including: #SPARQL #SQL #KnowledgeGraph #SemanticWeb #LinkedData #ODBC #JDBC #VirtuosoRDBMS demos & use cases:""" ;
	skos:related <https://twitter.com/hashtag/SPARQL#this> , <https://twitter.com/hashtag/SQL#this> , <https://twitter.com/hashtag/KnowledgeGraph#this> , <https://twitter.com/hashtag/SemanticWeb#this> , <https://twitter.com/hashtag/LinkedData#this> , <https://twitter.com/hashtag/ODBC#this> , <https://twitter.com/hashtag/JDBC#this> , <https://twitter.com/hashtag/VirtuosoRDBMS#this> , <http://data.openlinksw.com/oplweb/glossary-term/SPARQL#this> , <http://data.openlinksw.com/oplweb/glossary-term/SQL#this> , <http://data.openlinksw.com/oplweb/glossary-term/KnowledgeGraph#this> , <http://data.openlinksw.com/oplweb/glossary-term/SemanticWeb#this> , <http://data.openlinksw.com/oplweb/glossary-term/LinkedData#this> , <http://data.openlinksw.com/oplweb/glossary-term/ODBC#this> , <http://data.openlinksw.com/oplweb/glossary-term/JDBC#this> , <http://data.openlinksw.com/oplweb/glossary-term/VirtuosoRDBMS#this> ;
	rdfs:comment """Here is  @OpenLink
 weekly recap of some of last weeks activities covering a range of topics including: #SPARQL #SQL #KnowledgeGraph #SemanticWeb #LinkedData #ODBC #JDBC #VirtuosoRDBMS demos & use cases:""" .

<https://twitter.com/shewardmills/status/1174650044773031937#> a schema:CreativeWork , foaf:Document ;
	schema:url <https://twitter.com/shewardmills/status/1174650044773031937> ;
	schema:name "@EU_DataPortal:  Iceland" ;
	skos:related <https://twitter.com/hashtag/LinkedData#this> , <https://twitter.com/hashtag/KnowledgeGraph#this> , <http://ecrm.intranet.openlinksw.com/us_mis_csv#https%3A%2F%2Ftwitter.com%2Fhashtag%2FVirtuosoRDBMS+%23this> , <https://twitter.com/hashtag/OpenData#this> , <https://twitter.com/hashtag/Dataset#this> , <http://data.openlinksw.com/oplweb/glossary-term/LinkedData#this> , <http://data.openlinksw.com/oplweb/glossary-term/KnowledgeGraph#this> , <http://data.openlinksw.com/oplweb/glossary-term/VirtuosoRDBMS#this> , <http://data.openlinksw.com/oplweb/glossary-term/OpenData#this> , <http://data.openlinksw.com/oplweb/glossary-term/Dataset#this> ;
	rdfs:comment "@EU_DataPortal:  Iceland" .

<https://twitter.com/EmekaOkoye/status/1174334240156266496#> a schema:CreativeWork , foaf:Document ;
	schema:url <https://twitter.com/EmekaOkoye/status/1174334240156266496> ;
	schema:name """Retweet @EmekaOkoye:  Sample model of Lagos bus stops/routes using #RDF.

#SPARQL can be use to create queries on bus stops/routes and create CSV notations for #Algorithms to be applied.

#LinkedData easily makes cities computational so as to improve people���s lives, city operations and
environment. /7""" ;
	skos:related <https://twitter.com/hashtag/RDF#this> , <https://twitter.com/hashtag/SPARQL#this> , <https://twitter.com/hashtag/Algorithms#this> , <https://twitter.com/hashtag/LinkedData#this> , <http://data.openlinksw.com/oplweb/glossary-term/RDF#this> , <http://data.openlinksw.com/oplweb/glossary-term/SPARQL#this> , <http://data.openlinksw.com/oplweb/glossary-term/Algorithms#this> , <http://data.openlinksw.com/oplweb/glossary-term/LinkedData#this> ;
	rdfs:comment """Retweet @EmekaOkoye:  Sample model of Lagos bus stops/routes using #RDF.

#SPARQL can be use to create queries on bus stops/routes and create CSV notations for #Algorithms to be applied.

#LinkedData easily makes cities computational so as to improve people���s lives, city operations and
environment. /7""" .

<https://twitter.com/CarolineIdehen/status/1174674003673440257#> a schema:CreativeWork , foaf:Document ;
	schema:url <https://twitter.com/CarolineIdehen/status/1174674003673440257> ;
	schema:name """@OpenLink
 provides secure & high performance #ODBC, #JDBC, http://ADO.NET and #OLEDB drivers for #ProgressSW version 7.x all the way up to the latest #OpenEdge releases. 

Obtain a Free Trial at:  https://shop.openlinksw.com""" ;
	skos:related <https://twitter.com/hashtag/ODBC#this> , <https://twitter.com/hashtag/JDBC#this> , <https://twitter.com/hashtag/ADO.NET#this> , <https://twitter.com/hashtag/OLEDB#this> , <https://twitter.com/hashtag/ProgressSW#this> , <https://twitter.com/hashtag/OpenEdge#this> , <http://data.openlinksw.com/oplweb/glossary-term/ODBC#this> , <http://data.openlinksw.com/oplweb/glossary-term/JDBC#this> , <http://data.openlinksw.com/oplweb/glossary-term/ADO.NET#this> , <http://data.openlinksw.com/oplweb/glossary-term/OLEDB#this> , <http://data.openlinksw.com/oplweb/glossary-term/ProgressSW#this> , <http://data.openlinksw.com/oplweb/glossary-term/OpenEdge#this> ;
	rdfs:comment """@OpenLink
 provides secure & high performance #ODBC, #JDBC, http://ADO.NET and #OLEDB drivers for #ProgressSW version 7.x all the way up to the latest #OpenEdge releases. 

Obtain a Free Trial at:  https://shop.openlinksw.com""" .

<https://twitter.com/dan_hmills/status/1173604335806296065#> a schema:CreativeWork , foaf:Document ;
	schema:url <https://twitter.com/dan_hmills/status/1173604335806296065> ;
	schema:name "(2/3) And then copying the URL generated in your address bar. which can be bookmarked, or sent to somebody else ..." ;
	skos:related <https://twitter.com/hashtag/LinkedData#this> , <https://twitter.com/hashtag/GraphDatabases#this> , <https://twitter.com/hashtag/VirtuosoRDBMS#this> , <https://twitter.com/hashtag/SPARQL#this> , <http://data.openlinksw.com/oplweb/glossary-term/LinkedData#this> , <http://data.openlinksw.com/oplweb/glossary-term/GraphDatabases#this> , <http://data.openlinksw.com/oplweb/glossary-term/VirtuosoRDBMS#this> , <http://data.openlinksw.com/oplweb/glossary-term/SPARQL#this> ;
	rdfs:comment "(2/3) And then copying the URL generated in your address bar. which can be bookmarked, or sent to somebody else ..." .

<https://twitter.com/dan_hmills/status/1173604344803057669#> a schema:CreativeWork , foaf:Document ;
	schema:url <https://twitter.com/dan_hmills/status/1173604344803057669> ;
	schema:name """(3/3)

The URL can also be obtained by right clicking on the \"Permalink\" hyperlink, and copying the resulting link.""" ;
	skos:related <https://twitter.com/hashtag/LinkedData#this> , <https://twitter.com/hashtag/GraphDatabases#this> , <https://twitter.com/hashtag/VirtuosoRDBMS#this> , <https://twitter.com/hashtag/SPARQL#this> , <http://data.openlinksw.com/oplweb/glossary-term/LinkedData#this> , <http://data.openlinksw.com/oplweb/glossary-term/GraphDatabases#this> , <http://data.openlinksw.com/oplweb/glossary-term/VirtuosoRDBMS#this> , <http://data.openlinksw.com/oplweb/glossary-term/SPARQL#this> ;
	rdfs:comment """(3/3)

The URL can also be obtained by right clicking on the \"Permalink\" hyperlink, and copying the resulting link.""" .

<https://twitter.com/dan_hmills/status/1173624192459333633#> a schema:CreativeWork , foaf:Document ;
	schema:url <https://twitter.com/dan_hmills/status/1173624192459333633> ;
	schema:name """Replying to 
@datao
(1/2)
This skin for /SPARQL is only for the commercial edition. Permalinks can be made in the open source edition by executing the query and changing the \"query\" parameter to  'qtxt', and copy/pasting or sending the resulting URI.""" ;
	rdfs:comment """Replying to 
@datao
(1/2)
This skin for /SPARQL is only for the commercial edition. Permalinks can be made in the open source edition by executing the query and changing the \"query\" parameter to  'qtxt', and copy/pasting or sending the resulting URI.""" .

<https://twitter.com/dan_hmills/status/1173624922775703555#> a schema:CreativeWork , foaf:Document ;
	schema:url <https://twitter.com/dan_hmills/status/1173624922775703555> ;
	schema:name """Replying to 
@dan_hmills
 and 
@datao
(2/2)

Sample URI that uses this alternative approach from your SPARQL endpoint: https://tinyurl.com/y3zcnoqr""" ;
	rdfs:comment """Replying to 
@dan_hmills
 and 
@datao
(2/2)

Sample URI that uses this alternative approach from your SPARQL endpoint: https://tinyurl.com/y3zcnoqr""" .

<https://twitter.com/dan_hmills/status/1173638905721249794#> a schema:CreativeWork , foaf:Document ;
	schema:url <https://twitter.com/dan_hmills/status/1173638905721249794> ;
	schema:name """Replying to 
@col1m
 and 
@datao
@colm1
 Nice. How do I share a link to this page containing a query to somebody else? 

Also note that the output format selected in Virtuoso in the same manner by changing the 'output' parameter, and also by choosing a preferred output using /SPARQL's dropdown menu""" ;
	rdfs:comment """Replying to 
@col1m
 and 
@datao
@colm1
 Nice. How do I share a link to this page containing a query to somebody else? 

Also note that the output format selected in Virtuoso in the same manner by changing the 'output' parameter, and also by choosing a preferred output using /SPARQL's dropdown menu""" .

<https://twitter.com/kidehen/status/1174721625046036480#> a schema:CreativeWork , foaf:Document ;
	schema:url <https://twitter.com/kidehen/status/1174721625046036480> ;
	schema:name """Replying to 
@vrandezo
 and 
@chekovf
Why is there are need to knock #SPARQL when talking about #GQL, #Cypher etc..

A need to knock #RDF #DBMS and Stores when talking about a #GraphDatabase etc..

Everything should live or die by its own merits or demerits.

We now have a strange \"Label\" vs #Concept war raging :)""" ;
	skos:related <https://twitter.com/hashtag/SPARQL#this> , <https://twitter.com/hashtag/GQL#this> , <https://twitter.com/hashtag/Cypher#this> , <https://twitter.com/hashtag/RDF#this> , <https://twitter.com/hashtag/DBMS#this> , <https://twitter.com/hashtag/GraphDatabase#this> , <https://twitter.com/hashtag/Concept#this> , <http://data.openlinksw.com/oplweb/glossary-term/SPARQL#this> , <http://data.openlinksw.com/oplweb/glossary-term/GQL#this> , <http://data.openlinksw.com/oplweb/glossary-term/Cypher#this> , <http://data.openlinksw.com/oplweb/glossary-term/RDF#this> , <http://data.openlinksw.com/oplweb/glossary-term/DBMS#this> , <http://data.openlinksw.com/oplweb/glossary-term/GraphDatabase#this> , <http://data.openlinksw.com/oplweb/glossary-term/Concept#this> ;
	rdfs:comment """Replying to 
@vrandezo
 and 
@chekovf
Why is there are need to knock #SPARQL when talking about #GQL, #Cypher etc..

A need to knock #RDF #DBMS and Stores when talking about a #GraphDatabase etc..

Everything should live or die by its own merits or demerits.

We now have a strange \"Label\" vs #Concept war raging :)""" .

<https://twitter.com/kidehen/status/1174775577192148994#> a schema:CreativeWork , foaf:Document ;
	schema:url <https://twitter.com/kidehen/status/1174775577192148994> ;
	schema:name "1/2: Starting page: http://scihi.org/congress-of-vienna/ which has #SPARQL behind the page: https://tinyurl.com/y4u8z3qc. This is the kind of #DataConnectivity enabled by #LinkedData - when a #Hyperlink functions as a #SuperKey." ;
	skos:related <https://twitter.com/hashtag/SPARQL#this> , <https://twitter.com/hashtag/DataConnectivity#this> , <https://twitter.com/hashtag/LinkedData#this> , <https://twitter.com/hashtag/Hyperlink#this> , <https://twitter.com/hashtag/SuperKey#this> , <https://twitter.com/hashtag/KnowledgeGraph#this> , <https://twitter.com/hashtag/GraphDatabase#this> , <https://twitter.com/hashtag/Wikidata#this> , <https://twitter.com/hashtag/DBpedia#this> , <https://twitter.com/hashtag/SemanticWeb#this> , <http://data.openlinksw.com/oplweb/glossary-term/SPARQL#this> , <http://data.openlinksw.com/oplweb/glossary-term/DataConnectivity#this> , <http://data.openlinksw.com/oplweb/glossary-term/LinkedData#this> , <http://data.openlinksw.com/oplweb/glossary-term/Hyperlink#this> , <http://data.openlinksw.com/oplweb/glossary-term/SuperKey#this> , <http://data.openlinksw.com/oplweb/glossary-term/KnowledgeGraph#this> , <http://data.openlinksw.com/oplweb/glossary-term/GraphDatabase#this> , <http://data.openlinksw.com/oplweb/glossary-term/Wikidata#this> , <http://data.openlinksw.com/oplweb/glossary-term/DBPedia#this> , <http://data.openlinksw.com/oplweb/glossary-term/SemanticWeb#this> ;
	rdfs:comment "1/2: Starting page: http://scihi.org/congress-of-vienna/ which has #SPARQL behind the page: https://tinyurl.com/y4u8z3qc. This is the kind of #DataConnectivity enabled by #LinkedData - when a #Hyperlink functions as a #SuperKey." .

<https://twitter.com/kidehen/status/1174777492663652354#> a schema:CreativeWork , foaf:Document ;
	schema:url <https://twitter.com/kidehen/status/1174777492663652354> ;
	schema:name "2/2: I tweaked the #SPARQL behind the page: https://tinyurl.com/y5cfokts I published a new #Meshup using our #PivotViewer: https://tinyurl.com/y3nx96p3 -- over additional views and drill-down paths" ;
	skos:related <https://twitter.com/hashtag/SPARQL#this> , <https://twitter.com/hashtag/Meshup#this> , <https://twitter.com/hashtag/PivotViewer#this> , <https://twitter.com/hashtag/KnowledgeGraph#this> , <https://twitter.com/hashtag/GraphDatabase#this> , <https://twitter.com/hashtag/Wikidata#this> , <https://twitter.com/hashtag/DBpedia#this> , <https://twitter.com/hashtag/SemanticWeb#this> , <https://twitter.com/hashtag/VirtuosoRDBMS#this> , <https://twitter.com/hashtag/LODCloud#this> , <http://data.openlinksw.com/oplweb/glossary-term/SPARQL#this> , <http://data.openlinksw.com/oplweb/glossary-term/Meshup#this> , <http://data.openlinksw.com/oplweb/glossary-term/PivotViewer#this> , <http://data.openlinksw.com/oplweb/glossary-term/KnowledgeGraph#this> , <http://data.openlinksw.com/oplweb/glossary-term/GraphDatabase#this> , <http://data.openlinksw.com/oplweb/glossary-term/Wikidata#this> , <http://data.openlinksw.com/oplweb/glossary-term/DBPedia#this> , <http://data.openlinksw.com/oplweb/glossary-term/SemanticWeb#this> , <http://data.openlinksw.com/oplweb/glossary-term/VirtuosoRDBMS#this> , <http://data.openlinksw.com/oplweb/glossary-term/LODCloud#this> ;
	rdfs:comment "2/2: I tweaked the #SPARQL behind the page: https://tinyurl.com/y5cfokts I published a new #Meshup using our #PivotViewer: https://tinyurl.com/y3nx96p3 -- over additional views and drill-down paths" .

<https://twitter.com/kidehen/status/1174786137694621701#> a schema:CreativeWork , foaf:Document ;
	schema:url <https://twitter.com/kidehen/status/1174786137694621701> ;
	schema:name """More #LinkedData utility demos from the UK Ordnance Survey. @datasniff
 also demonstrates use of #HTML5-based #StructuredData islands using #RDFa.""" ;
	skos:related <https://twitter.com/hashtag/LinkedData#this> , <https://twitter.com/hashtag/HTML5#this> , <https://twitter.com/hashtag/StructuredData#this> , <https://twitter.com/hashtag/RDFa#this> , <https://twitter.com/hashtag/GraphDatabase#this> , <https://twitter.com/hashtag/KnowledgeGraph#this> , <http://ecrm.intranet.openlinksw.com/us_mis_csv#https%3A%2F%2Ftwitter.com%2Fhashtag%2FCDO%0ADataOps%23this> , <https://twitter.com/hashtag/ConnectedData#this> , <https://twitter.com/hashtag/LODCloud#this> , <http://data.openlinksw.com/oplweb/glossary-term/LinkedData#this> , <http://data.openlinksw.com/oplweb/glossary-term/HTML5#this> , <http://data.openlinksw.com/oplweb/glossary-term/StructuredData#this> , <http://data.openlinksw.com/oplweb/glossary-term/RDFa#this> , <http://data.openlinksw.com/oplweb/glossary-term/GraphDatabase#this> , <http://data.openlinksw.com/oplweb/glossary-term/KnowledgeGraph#this> , <http://data.openlinksw.com/oplweb/glossary-term/CDO#this> , <http://data.openlinksw.com/oplweb/glossary-term/DataOps#this> , <http://data.openlinksw.com/oplweb/glossary-term/ConnectedData#this> , <http://data.openlinksw.com/oplweb/glossary-term/LODCloud#this> ;
	rdfs:comment """More #LinkedData utility demos from the UK Ordnance Survey. @datasniff
 also demonstrates use of #HTML5-based #StructuredData islands using #RDFa.""" .

<https://twitter.com/kidehen/status/1175079038223888387#> a schema:CreativeWork , foaf:Document ;
	schema:url <https://twitter.com/kidehen/status/1175079038223888387> ;
	schema:name """Replying to 
@EmekaOkoye
 
@AlanMorrison
 and 4 others
That article has a point of unclarity the permeates the entire piece. For instance, the term \"semantics\" is disconnected from \"context\". 

It is the fidelity of \"Entity Relationship Type Semantics\" that determines the contextual richness of any content.""" ;
	skos:related <https://twitter.com/hashtag/LinkedData#this> , <https://twitter.com/hashtag/SemanticWeb#this> , <http://data.openlinksw.com/oplweb/glossary-term/LinkedData#this> , <http://data.openlinksw.com/oplweb/glossary-term/SemanticWeb#this> ;
	rdfs:comment """Replying to 
@EmekaOkoye
 
@AlanMorrison
 and 4 others
That article has a point of unclarity the permeates the entire piece. For instance, the term \"semantics\" is disconnected from \"context\". 

It is the fidelity of \"Entity Relationship Type Semantics\" that determines the contextual richness of any content.""" .

<https://twitter.com/kidehen/status/1175120363249983488#> a schema:CreativeWork , foaf:Document ;
	schema:url <https://twitter.com/kidehen/status/1175120363249983488> ;
	schema:name """Replying to 
@ayooladejo
Tip:
Mentioning folks using their #DBpedia ID provides an entry point into a world of discovery provided by the #LODCloud #KnowledgeGraph.
Examples:
1. Kunle Afolayan 
2. Genevieve_Nnaji """ ;
	skos:related <https://twitter.com/hashtag/DBpedia#this> , <https://twitter.com/hashtag/LODCloud#this> , <https://twitter.com/hashtag/KnowledgeGraph#this> , <https://twitter.com/hashtag/Nollywood#this> , <https://twitter.com/hashtag/LinkedData#this> , <https://twitter.com/hashtag/GraphDatabase#this> , <http://data.openlinksw.com/oplweb/glossary-term/DBPedia#this> , <http://data.openlinksw.com/oplweb/glossary-term/LODCloud#this> , <http://data.openlinksw.com/oplweb/glossary-term/KnowledgeGraph#this> , <http://data.openlinksw.com/oplweb/glossary-term/Nollywood#this> , <http://data.openlinksw.com/oplweb/glossary-term/LinkedData#this> , <http://data.openlinksw.com/oplweb/glossary-term/GraphDatabase#this> ;
	rdfs:comment """Replying to 
@ayooladejo
Tip:
Mentioning folks using their #DBpedia ID provides an entry point into a world of discovery provided by the #LODCloud #KnowledgeGraph.
Examples:
1. Kunle Afolayan 
2. Genevieve_Nnaji """ ;
	schema:name "Simple #SocialNetwork Graph Analytics using our #VirtuosoRDBMS which combines the best of #SPARQL and #SQL. Sampling of connections centered around my #WebID combined with the contact network size per connected individual:" ;
	skos:related <https://twitter.com/hashtag/SocialNetwork#this> , <https://twitter.com/hashtag/VirtuosoRDBMS#this> , <https://twitter.com/hashtag/SPARQL#this> , <https://twitter.com/hashtag/SQL#this> , <https://twitter.com/hashtag/WebID#this> , <http://data.openlinksw.com/oplweb/glossary-term/SocialNetwork#this> , <http://data.openlinksw.com/oplweb/glossary-term/VirtuosoRDBMS#this> , <http://data.openlinksw.com/oplweb/glossary-term/SPARQL#this> , <http://data.openlinksw.com/oplweb/glossary-term/SQL#this> , <http://data.openlinksw.com/oplweb/glossary-term/WebID#this> ;
	rdfs:comment "Simple #SocialNetwork Graph Analytics using our #VirtuosoRDBMS which combines the best of #SPARQL and #SQL. Sampling of connections centered around my #WebID combined with the contact network size per connected individual:" .

<https://twitter.com/kidehen/status/1175450712597245952#> a schema:CreativeWork , foaf:Document ;
	schema:url <https://twitter.com/kidehen/status/1175450712597245952> ;
	schema:name """Retweet Linked Data Patterns
@datapatterns
Follow Your Nose - How do we find additional relevant data from the web?""" ;
	skos:related <https://twitter.com/hashtag/LinkedData#this> , <http://data.openlinksw.com/oplweb/glossary-term/LinkedData#this> ;
	rdfs:comment """Retweet Linked Data Patterns
@datapatterns
Follow Your Nose - How do we find additional relevant data from the web?""" .

<https://twitter.com/kidehen/status/1175500571266166786#> a schema:CreativeWork , foaf:Document ;
	schema:url <https://twitter.com/kidehen/status/1175500571266166786> ;
	schema:name """Replying to 
@kidehen
 
@EmekaOkoye
 and 5 others
That article has a point of unclarity that permeates the entire piece. For instance, the term \"semantics\" is disconnected from \"context\". 

It is the fidelity of \"Entity Relationship Type Semantics\" that determines the contextual richness of any content.""" ;
	skos:related <https://twitter.com/hashtag/LinkedData#this> , <https://twitter.com/hashtag/SemanticWeb#this> , <http://data.openlinksw.com/oplweb/glossary-term/LinkedData#this> , <http://data.openlinksw.com/oplweb/glossary-term/SemanticWeb#this> ;
	rdfs:comment """Replying to 
@kidehen
 
@EmekaOkoye
 and 5 others
That article has a point of unclarity that permeates the entire piece. For instance, the term \"semantics\" is disconnected from \"context\". 

It is the fidelity of \"Entity Relationship Type Semantics\" that determines the contextual richness of any content.""" .

<https://twitter.com/kidehen/status/1175541715672940544#> a schema:CreativeWork , foaf:Document ;
	schema:url <https://twitter.com/kidehen/status/1175541715672940544> ;
	schema:name "Looking at the #DBWik, a #KnowledgeGraph constructed from thousands of Wikis. See: http://dbkwik.webdatacommons.org" ;
	skos:related <https://twitter.com/hashtag/DBWik#this> , <https://twitter.com/hashtag/KnowledgeGraph#this> , <https://twitter.com/hashtag/GraphDatabase#this> , <https://twitter.com/hashtag/SPARQL#this> , <https://twitter.com/hashtag/VirtuosoRDBMS#this> , <https://twitter.com/hashtag/SemanticWeb#this> , <https://twitter.com/hashtag/CDO#this> , <https://twitter.com/hashtag/DataOps#this> , <https://twitter.com/hashtag/LODCloud#this> , <https://twitter.com/hashtag/DBpedia#this> , <http://data.openlinksw.com/oplweb/glossary-term/DBWik#this> , <http://data.openlinksw.com/oplweb/glossary-term/KnowledgeGraph#this> , <http://data.openlinksw.com/oplweb/glossary-term/GraphDatabase#this> , <http://data.openlinksw.com/oplweb/glossary-term/SPARQL#this> , <http://data.openlinksw.com/oplweb/glossary-term/VirtuosoRDBMS#this> , <http://data.openlinksw.com/oplweb/glossary-term/SemanticWeb#this> , <http://data.openlinksw.com/oplweb/glossary-term/CDO#this> , <http://data.openlinksw.com/oplweb/glossary-term/DataOps#this> , <http://data.openlinksw.com/oplweb/glossary-term/LODCloud#this> , <http://data.openlinksw.com/oplweb/glossary-term/DBPedia#this> ;
	rdfs:comment "Looking at the #DBWik, a #KnowledgeGraph constructed from thousands of Wikis. See: http://dbkwik.webdatacommons.org" .

<https://twitter.com/kidehen/status/1175542980465369089#> a schema:CreativeWork , foaf:Document ;
	schema:url <https://twitter.com/kidehen/status/1175542980465369089> ;
	schema:name """Replying to 
@AlanMorrison
 
@EmekaOkoye
 and 4 others
Twitter thread management #UI has introduced some confusion here. 

My comments where directed toward the other post shared by @EmekaOkoye
.

As for Multiple Models: 
I am anti-monoculture by nature so I have nothing against their existence and coherent use :)""" ;
	skos:related <https://twitter.com/hashtag/UI#this> , <http://data.openlinksw.com/oplweb/glossary-term/UI#this> ;
	rdfs:comment """Replying to 
@AlanMorrison
 
@EmekaOkoye
 and 4 others
Twitter thread management #UI has introduced some confusion here. 

My comments where directed toward the other post shared by @EmekaOkoye
.

As for Multiple Models: 
I am anti-monoculture by nature so I have nothing against their existence and coherent use :)""" .

<https://twitter.com/kidehen/status/1175544164005634048#> a schema:CreativeWork , foaf:Document ;
	schema:url <https://twitter.com/kidehen/status/1175544164005634048> ;
	schema:name """Replying to 
@kidehen
 
@AlanMorrison
 and 5 others
The post identified by the URL: https://simplea.com/Articles/structure-and-semantics-for-context
, is the target of my comments about artificial separation of \"semantics\" and \"context\". 

\"Entity Relationship Type Semantics\" are the keys to \"Content Context\"""" ;
	skos:related <https://twitter.com/hashtag/SemanticWeb#this> , <https://twitter.com/hashtag/KnowledgeGraph#this> , <http://data.openlinksw.com/oplweb/glossary-term/SemanticWeb#this> , <http://data.openlinksw.com/oplweb/glossary-term/KnowledgeGraph#this> ;
	rdfs:comment """Replying to 
@kidehen
 
@AlanMorrison
 and 5 others
The post identified by the URL: https://simplea.com/Articles/structure-and-semantics-for-context
, is the target of my comments about artificial separation of \"semantics\" and \"context\". 

\"Entity Relationship Type Semantics\" are the keys to \"Content Context\"""" .

<https://twitter.com/kidehen/status/1175587043801468928#> a schema:CreativeWork , foaf:Document ;
	schema:url <https://twitter.com/kidehen/status/1175587043801468928> .

<https://twitter.com/kidehen/status/1175587343304200192#> a schema:CreativeWork , foaf:Document ;
	schema:url <https://twitter.com/kidehen/status/1175587343304200192> ;
	schema:name """Retweet Margaret Warren
@ImageSnippets
When you search for images with Imagesnippets, it demonstrates inference and graphs that have been built with inference from #dbpedia and #wikidata @wikidata
 @dbpedia""" ;
	skos:related <https://twitter.com/hashtag/LinkedData#this> , <https://twitter.com/hashtag/SemanticWeb#this> , <https://twitter.com/hashtag/Wikidata#this> , <https://twitter.com/hashtag/DBPedia#this> , <http://data.openlinksw.com/oplweb/glossary-term/LinkedData#this> , <http://data.openlinksw.com/oplweb/glossary-term/SemanticWeb#this> , <http://data.openlinksw.com/oplweb/glossary-term/Wikidata#this> , <http://data.openlinksw.com/oplweb/glossary-term/DBPedia#this> ;
	rdfs:comment """Retweet Margaret Warren
@ImageSnippets
When you search for images with Imagesnippets, it demonstrates inference and graphs that have been built with inference from #dbpedia and #wikidata @wikidata
 @dbpedia""" .

<https://twitter.com/OpenLink/status/1174743452023701505#> a schema:CreativeWork , foaf:Document ;
	schema:url <https://twitter.com/OpenLink/status/1174743452023701505> ;
	schema:name "What are the basics of #LinkedData?" ;
	skos:related <https://twitter.com/hashtag/LinkedData#this> , <https://twitter.com/hashtag/KnowledgeGraph#this> , <http://data.openlinksw.com/oplweb/glossary-term/LinkedData#this> , <http://data.openlinksw.com/oplweb/glossary-term/KnowledgeGraph#this> ;
	rdfs:comment "What are the basics of #LinkedData?" .

<https://twitter.com/OpenLink/status/1175032849717768198#> a schema:CreativeWork , foaf:Document ;
	schema:url <https://twitter.com/OpenLink/status/1175032849717768198> ;
	schema:name "Making an #ODBC Connection from macOS to #PostgreSQL on #Azure:" ;
	skos:related <https://twitter.com/hashtag/ODBC#this> , <https://twitter.com/hashtag/PostgreSQL#this> , <https://twitter.com/hashtag/Azure#this> , <http://data.openlinksw.com/oplweb/glossary-term/ODBC#this> , <http://data.openlinksw.com/oplweb/glossary-term/PostgreSQL#this> , <http://data.openlinksw.com/oplweb/glossary-term/Azure#this> ;
	rdfs:comment "Making an #ODBC Connection from macOS to #PostgreSQL on #Azure:" .

<https://twitter.com/EmekaOkoye/status/1174013688401006592#> a schema:CreativeWork , foaf:Document ;
	schema:url <https://twitter.com/EmekaOkoye/status/1174013688401006592> ;
	schema:name """Retweet Emeka Azuka Okoye
@EmekaOkoye
Let me share what i learnt from one of my mentors @kidehen
 eons ago:

Developers are not real world problem domain experts. Hence their orientation towards building rip and replace apps.""" ;
	rdfs:comment """Retweet Emeka Azuka Okoye
@EmekaOkoye
Let me share what i learnt from one of my mentors @kidehen
 eons ago:

Developers are not real world problem domain experts. Hence their orientation towards building rip and replace apps.""" .

<https://twitter.com/OpenLink/status/1151982237245673478#> a schema:CreativeWork , foaf:Document ;
	schema:url <https://twitter.com/OpenLink/status/1151982237245673478> ;
	schema:name "Q: Can I use both #SPARQL and #SQL as query languages for operating on data managed by a #VirtuosoRDBMS instance?" ;
	skos:related <https://twitter.com/hashtag/SPARQL#this> , <https://twitter.com/hashtag/SQL#this> , <https://twitter.com/hashtag/VirtuosoRDBMS#this> , <https://twitter.com/hashtag/DBpedia#this> , <https://twitter.com/hashtag/Wikidata#this> , <https://twitter.com/hashtag/LODCloud#this> , <https://twitter.com/hashtag/ODBC#this> , <https://twitter.com/hashtag/JDBC#this> , <https://twitter.com/hashtag/DotNET#this> , <https://twitter.com/hashtag/GraphDatabase#this> , <https://twitter.com/hashtag/NoSQL#this> , <http://data.openlinksw.com/oplweb/glossary-term/SPARQL#this> , <http://data.openlinksw.com/oplweb/glossary-term/SQL#this> , <http://data.openlinksw.com/oplweb/glossary-term/VirtuosoRDBMS#this> , <http://data.openlinksw.com/oplweb/glossary-term/DBPedia#this> , <http://data.openlinksw.com/oplweb/glossary-term/Wikidata#this> , <http://data.openlinksw.com/oplweb/glossary-term/LODCloud#this> , <http://data.openlinksw.com/oplweb/glossary-term/ODBC#this> , <http://data.openlinksw.com/oplweb/glossary-term/JDBC#this> , <http://data.openlinksw.com/oplweb/glossary-term/DotNet#this> , <http://data.openlinksw.com/oplweb/glossary-term/GraphDatabase#this> , <http://data.openlinksw.com/oplweb/glossary-term/NoSQL#this> ;
	rdfs:comment "Q: Can I use both #SPARQL and #SQL as query languages for operating on data managed by a #VirtuosoRDBMS instance?" .
